Correctness-proof for GodelT

_in/textbook/DemoTextbook.lean
@@ -11,6 +11,7 @@ open Verso.Genre Manual
 open DemoTextbook.Exts (lean)
 
 set_option pp.rawOnError true
+set_option maxRecDepth 1000
 
 #doc (Manual) "Normalization by Evaluation in Lean4" =>
 
@@ -205,7 +206,7 @@ theorem app_eval (a : Exp α) : ∀ b, (a ⬝ b) ~ (eval a b) :=
 
 ## Reification
 
-Now that we can evaluate out Monoid-expressions such that they're normalized at the Meta-level, how do we bring them back down to the object-level such that we don't change the "behavior" (wrt `~`)?
+Now that we can evaluate our Monoid-expressions such that they're normalized at the Meta-level, how do we bring them back down to the object-level such that we don't change the "behavior" (wrt `~`)?
 Well, for a given `e : Exp α`, we intuitively know that `eval e : Exp α → Exp α` will have the form:
 
 `λ e' ↦ elem x₁ ⬝ (elem x₂ ⬝ ... ⬝ (elem xₙ ⬝ e'))`
@@ -227,12 +228,26 @@ def nbe (e : Exp α) : Exp α := reify (eval e)
 What `nbe` does is first evaluate `e` so it gets normalized through function-composition, and then reify's it back into a canonical element of `[e]~`.
 Thus, we can translate `a ~ b` into the decidable-problem `nbe a = nbe b` which we state as our main correctness-theorem:
 
+`(e ~ e') ↔ (nbe e = nbe e')`
+
+Before we move onto the proof of correctness, we introduce an additional key lemma showing nbe really does return a element of `[e]~`:
+
 ```lean
-theorem correctness (e e' : Exp α) : (e ~ e') ↔ (nbe e = nbe e') :=
+theorem convr_nbe (e : Exp α) : e ~ (nbe e) :=
+  by
+  sorry
+```
+[Try it!](https://live.lean-lang.org/#codez=JYWwDg9gTgLgBAWQIYwBYBtgCMB0AVJAYxmEICgyBaSuAMSghAC45UYYwBnJgeh8M45gEQjgCmYnmIDunATwBMABiUBOHgBMAnlgBWYqDxBJgAOwAKSdCE5jKUMQDdgtjTjAaAZhTMaArsTAjmJwAKIAHmBwABSAjcBwLHhaYGIAlGQAPnBIYFEsEVHxgEmEYZFwxaWFmXDAGnAJleXVYuhiIA0VBU1mnsDhDQCMKnAARHCAuNSjcAC8AHyVODlgFFQ0ACK1pgDk8BpihOhIDnBoIQDKYjAQtTWmnDBIpoQhntAnqC5wWpdkvgEkwTghAgpkcUAa0S6sVScBKkLK0NhcHMDGWWSQnE4IjgAG8QmItnACYT8giAL4NYGg8HRaIhSYEmEMrZbGF0iYxAkc4mpdJZWoAfVanngePqpMKFPq4qBILBMXhYCEGiZRLZaWqgqgwAA5mxcSEJeUpdKWFT5ezJgVleq+XAHJ50NL6mKjbETTLzTS0py7ZwtO1nQaiSTGu7PXLverWUivZyY3S7TAoI9OMGucSGlCKWbI774zCSnG6QmebG84n46zqktcUg4FggXA6m6PbnqTEkGysIXZR3ooQ2Sry/365NBzFG5MVb9TL1+iwhkopgA/KZzPtglZ7TxExxWCFQ3uK8pIo9kepZa21+uNjfRQDdwESZvMnAf63T907G2l0peFjcQYbrUF5wFekTiK07T9C+MRPiE97Wi0bRwOEqoahQ1DZHAa6Nkib5OvW0x7geWBkFBxiblAAoETRACOdYNlm5IxKgDT1rhMIsIAAERAgANJyX7ZDChD1MRn6kSJCTTGQWBaKBfyBCCrCgY8WgCjqEBWJwoH1GYyYQJwADc2RiFiyygYQGIhDeTGiXUApwI5SBYAKwBsYQGhuWxcy6UCrRHHAABUcA0C53lAl57l+fpDBEn5nApIQwBWMAABeISeRFYgJUlKWYBl2Sue5CoEc2MIas6nCgFEILoFocAANoEQAun5UDSE1WXuW1zodU14U9ZhNC8VgAljkxa4SYRDbpBR9ZLDRQnRPWbpcXAo0CStHI9jhgnvrN0myfJemmP4SmmNklnWdkuRNnUhARVFPmzDFpgGQ2fl+HOEDoHUBG5fs+XpSEz2fVVeWpYVj0ldNzazX5qBIICqDLiwtKidOqq7VNmMxHUkw9lxxFeosmIiO1Yi9KYIQDpGODJqmrDLgA/AKf7SgcYiBajiPIyEqMQnj0QE7NMK4xycN1ET0lUYsd109SOAOugQ7eRz9QOmYtOk4zdzM3AbMa/53PgrzzpiOERDwDDqAUPUVm2DUdS+c6sUQOD0qW9bcuCsKMD20CN3Ie0rvSu7nv1N7xByyrFA7vaYjAJ4DXRLubpngi60noiTDEbu1ogWQCemFgtOGmG61QrLDjJ6nZUYfNVECqX5fMYU60hGurfPnnoFyaBWEABL6SwXfPpMNyD2FZ1wH4TuLQD9RYlAUBaEAA)
+[Solution](https://live.lean-lang.org/#codez=JYWwDg9gTgLgBAWQIYwBYBtgCMB0AVJAYxmEICgyBaSuAMSghAC45UYYwBnJgeh8M45gEQjgCmYnmIDunATwBMABiUBOHgBMAnlgBWYqDxBJgAOwAKSdCE5jKUMQDdgtjTjAaAZhTMaArsTAjmJwAKIAHmBwABSAjcBwLHhaYGIAlGQAPnBIYFEsEVHxgEmEYZFwxaWFmXDAGnAJleXVYuhiIA0VBU1mnsDhDQCMKnAARHCAuNSjcAC8AHyVODlgFFQ0ACK1pgDk8BpihOhIDnBoIQDKYjAQtTWmnDBIpoQhntAnqC5wWpdkvgEkwTghAgpkcUAa0S6sVScBKkLK0NhcHMDGWWSQnE4IjgAG8QmItnACYT8giAL4NYGg8HRaIhSYEmEMrZbGF0iYxAkc4mpdJZWoAfVanngePqpMKFPq4qBILBMXhYCEGiZRLZaWqgqgwAA5mxcSEJeUpdKWFT5ezJgVleq+XAHJ50NL6mKjbETTLzTS0py7ZwtO1nQaiSTGu7PXLverWUivZyY3S7TAoI9OMGucSGlCKWbI774zCSnG6QmebG84n46zqktcUg4FggXA6m6PbnqTEkGysIXZR3ooQ2Sry/365NBzFG5MVb9TL1+iwhkopgA/KZzPtglZ7TxExxWCFQ3uK8pIo9kepZa21+uNjfRQDdwESZvMnAf63T907G2l0peFjcQYbrUF5wFekTiK07T9C+MRPiE97Wi0bRwOEqoahQ1DZHAa6Nkib5OvW0x7geWBkFBxiblAAoETRACOdYNlm5IxKgDT1rhMIsIAAERAgANJyX7ZDChD1MRn6kSJCTTGQWBaKBfyBCCrCgY8WgCjqEBWJwoH1GYyYQJwADc2RiFiyygYQGIhDeTGiXUApwI5SBYAKwBsYQGhuWxcy6UCrRHHAABUcA0C53lAl57l+fpDBEn5nApIQwBWMAABeISeRFYgJUlKWYBl2Sue5CoEc2MIas6nCgFEILoFocAANoEQAun5UDSE1WXuW1zodU14U9ZhNC8VgAljkxa4SYRDbpBR9ZLDRQnRPWbpcXAo0CStHI9jhgnvrN0myfJemmP4SmmNklnWdkuRNnUhARVFPmzDFpgGQ2fl+HOEDoHUBG5fs+XpSEz2fVVeWpYVj0ldNzazX5qBIICqDLiwtKidOqq7VNmMxHUkw9lxxFeosmIiO1Yi9KYIQDpGODJqmrDLgA/AKf7SgcYiBajiPIyEqMQnj0QE7NMK4xycN1ET0lUYsd109SOAOugQ7eRz9QOmYtOk4zdzM3AbMa/53PgrzzpiOERDwDDqAUPUVm2DUdS+c6sUQOD0qW9bcuCsKMD20CN3Ie0rvSu7nv1N7xByyrFA7vaYjAJ4DXRLubpngi60noiTDEbu1ogWQCemFgtOGmG61QrLDjJ6nZUYfNVECqX5fMYU60hGurfPnnoFyaBSMo2jz5TfSAHDnnMSk/67Sk1qupsBzWs09P9N62mgtG5ZAVm0ooHR/Ai0NxPQA)
+
+We are now ready to prove our algorithm correct:
+
+```lean
+theorem correctness {e e' : Exp α} : (e ~ e') ↔ (nbe e = nbe e') :=
     by sorry
 ```
-[Try it!](https://live.lean-lang.org/#codez=JYWwDg9gTgLgBAWQIYwBYBtgCMB0AVJAYxmEICgyBaSuAMSghAC45UYYwBnJgeh8M45gEQjgCmYnmIDunATwBMABiUBOHgBMAnlgBWYqDxBJgAOwAKSdCE5jKUMQDdgtjTjAaAZhTMaArsTAjmJwAKIAHmBwABSAjcBwLHhaYGIAlGQAPnBIYFEsEVHxgEmEYZFwxaWFmXDAGnAJleXVYuhiIA0VBU1mnsDhDQCMKnAARHCAuNSjcAC8AHyVODlgFFQ0ACK1pgDk8BpihOhIDnBoIQDKYjAQtTWmnDBIpoQhntAnqC5wWpdkvgEkwTghAgpkcUAa0S6sVScBKkLK0NhcHMDGWWSQnE4IjgAG8QmItnACYT8giAL4NYGg8HRaIhSYEmEMrZbGF0iYxAkc4mpdJZWoAfVanngePqpMKFPq4qBILBMXhYCEGiZRLZaWqgqgwAA5mxcSEJeUpdKWFT5ezJgVleq+XAHJ50NL6mKjbETTLzTS0py7ZwtO1nQaiSTGu7PXLverWUivZyY3S7TAoI9OMGucSGlCKWbI774zCSnG6QmebG84n46zqktcUg4FggXA6m6PbnqTEkGysIXZR3ooQ2Sry/365NBzFG5MVb9TL1+iwhkopgA/KZzPtglZ7TxExxWCFQ3uK8pIo9kepZa21+uNjfRQDdwESZvMnAf63T907G2l0peFjcQYbrUF5wFekTiK07T9C+MRPiE97Wi0bRwOEqoahQ1DZHAa6Nkib5OvW0x7geWBkFBxiblAAoETRACOdYNlm5IxKgDT1rhMIsIAAERAgANJyX7ZDChD1MRn6kSJCTTGQWBaKBfyBCCrCgY8WgCjqEBWJwoH1GYyYQJwADc2RiFiyygYQGIhDeTGiXUApwI5SBYAKwBsYQGhuWxcy6UCrRHHAABUcA0C53lAl57l+fpDBEn5nApIQwBWMAABeISeRFYgJUlKWYBl2Sue5CoEc2MIas6nCgFEILoFocAANoEQAun5UDSE1WXuW1zodU14U9ZhNC8VgAljkxa4SYRDbpBR9ZLDRQnRPWbpcXAo0CStHI9jhgnvrN0myfJemmP4SmmNklnWdkuRNnUhARVFPmzDFpgGQ2fl+HOEDoHUBG5fs+XpSEz2fVVeWpYVj0ldNzazX5qBIICqDLiwtKidOqq7VNmMxHUkw9lxxFeosmIiO1Yi9KYIQDpGODJqmrDLgA/AKf7SgcYiBajiPIyEqMQnj0QE7NMK4xycN1ET0lUYsd109SOAOugQ7eRz9QOmYtOk4zdzM3AbMa/53PgrzzpiOERDwDDqAUPUVm2DUdS+c6sUQOD0qW9bcuCsKMD20CN3Ie0rvSu7nv1N7xByyrFA7vaYjAJ4DXRLubpngi60noiTDEbu1ogWQCemFgtOGmG61QrLDjJ6nZUYVhZyoBAsjNkDGgucAmAwA1EC7iEa4EmQpzQChwJQA4xA05inIhsxhTZ4PIYwoAKYQxKX+IzHAm8r0dcmqbk9VwAAkp4nhCO9DCgQA7bcH1227Z3/MIl2P9KakaVp6A6UGpnmX5R2IRwDyyiLee62QBTUUbI9aiDknIvj8g7AK4IQphSgQKGBGCNBINCjQAAEvpFgABVJ2XolpWHorgrEk95K3zgN9V4f0d5l0TnXN6D8lB+SwoQ96JCnaC0eHURaAMqrQCgFoIAA)
-[Solution](https://live.lean-lang.org/#codez=JYWwDg9gTgLgBAWQIYwBYBtgCMB0AVJAYxmEICgyBaSuAMSghAC45UYYwBnJgeh8M45gEQjgCmYnmIDunATwBMABiUBOHgBMAnlgBWYqDxBJgAOwAKSdCE5jKUMQDdgtjTjAaAZhTMaArsTAjmJwAKIAHmBwABSAjcBwLHhaYGIAlGQAPnBIYFEsEVHxgEmEYZFwxaWFmXDAGnAJleXVYuhiIA0VBU1mnsDhDQCMKnAARHCAuNSjcAC8AHyVODlgFFQ0ACK1pgDk8BpihOhIDnBoIQDKYjAQtTWmnDBIpoQhntAnqC5wWpdkvgEkwTghAgpkcUAa0S6sVScBKkLK0NhcHMDGWWSQnE4IjgAG8QmItnACYT8giAL4NYGg8HRaIhSYEmEMrZbGF0iYxAkc4mpdJZWoAfVanngePqpMKFPq4qBILBMXhYCEGiZRLZaWqgqgwAA5mxcSEJeUpdKWFT5ezJgVleq+XAHJ50NL6mKjbETTLzTS0py7ZwtO1nQaiSTGu7PXLverWUivZyY3S7TAoI9OMGucSGlCKWbI774zCSnG6QmebG84n46zqktcUg4FggXA6m6PbnqTEkGysIXZR3ooQ2Sry/365NBzFG5MVb9TL1+iwhkopgA/KZzPtglZ7TxExxWCFQ3uK8pIo9kepZa21+uNjfRQDdwESZvMnAf63T907G2l0peFjcQYbrUF5wFekTiK07T9C+MRPiE97Wi0bRwOEqoahQ1DZHAa6Nkib5OvW0x7geWBkFBxiblAAoETRACOdYNlm5IxKgDT1rhMIsIAAERAgANJyX7ZDChD1MRn6kSJCTTGQWBaKBfyBCCrCgY8WgCjqEBWJwoH1GYyYQJwADc2RiFiyygYQGIhDeTGiXUApwI5SBYAKwBsYQGhuWxcy6UCrRHHAABUcA0C53lAl57l+fpDBEn5nApIQwBWMAABeISeRFYgJUlKWYBl2Sue5CoEc2MIas6nCgFEILoFocAANoEQAun5UDSE1WXuW1zodU14U9ZhNC8VgAljkxa4SYRDbpBR9ZLDRQnRPWbpcXAo0CStHI9jhgnvrN0myfJemmP4SmmNklnWdkuRNnUhARVFPmzDFpgGQ2fl+HOEDoHUBG5fs+XpSEz2fVVeWpYVj0ldNzazX5qBIICqDLiwtKidOqq7VNmMxHUkw9lxxFeosmIiO1Yi9KYIQDpGODJqmrDLgA/AKf7SgcYiBajiPIyEqMQnj0QE7NMK4xycN1ET0lUYsd109SOAOugQ7eRz9QOmYtOk4zdzM3AbMa/53PgrzzpiOERDwDDqAUPUVm2DUdS+c6sUQOD0qW9bcuCsKMD20CN3Ie0rvSu7nv1N7xByyrFA7vaYjAJ4DXRLubpngi60noiTDEbu1ogWQCemFgtOGmG61QrLDjJ6nZUYVhZyoBAsjNkDGgucAmAwA1EC7iEa4EmQpzQChwJQA4xA05inIhsxhTZ4PIYwoAKYQxKX+IzHAm8r0dcmqbk9VwAAkp4nhCO9DCgQA7bcH1227Z3/MIl2P9KakaVp6A6UGpnmX5R2IRwDyyiLee62QBTUUbI9aiDknIvj8g7AK4IQphSgQKGBGCNBINYPzbIsDMEtk7ByCcU0pzlVlqTG8GCsFwNwdHG2kYlpWHogQ2hdRC44NvnAb6rw/o7zLonOub0H5KD5ijAYDRl6WgAsOPOMRSb+naKTLUuo2DGy1jTRR9M9ZplQFIo2gCUGsAGBIgWUj0b0jkeLUqQkfRcOJrdMALCnQhC4ZTamOtdEpn1gYw27NjGm1MZTaQ2oYAhEaqjXqnMTHm2lEjFGaM7EHkZDYvaJYOSOKofTZRnZciuPno4zx2sdFKz0QbIxzouY83ERbK2MdVFeW1HqGAQA)
+[Try it!](https://live.lean-lang.org/#codez=JYWwDg9gTgLgBAWQIYwBYBtgCMB0AVJAYxmEICgyBaSuAMSghAC45UYYwBnJgeh8M45gEQjgCmYnmIDunATwBMABiUBOHgBMAnlgBWYqDxBJgAOwAKSdCE5jKUMQDdgtjTjAaAZhTMaArsTAjmJwAKIAHmBwABSAjcBwLHhaYGIAlGQAPnBIYFEsEVHxgEmEYZFwxaWFmXDAGnAJleXVYuhiIA0VBU1mnsDhDQCMKnAARHCAuNSjcAC8AHyVODlgFFQ0ACK1pgDk8BpihOhIDnBoIQDKYjAQtTWmnDBIpoQhntAnqC5wWpdkvgEkwTghAgpkcUAa0S6sVScBKkLK0NhcHMDGWWSQnE4IjgAG8QmItnACYT8giAL4NYGg8HRaIhSYEmEMrZbGF0iYxAkc4mpdJZWoAfVanngePqpMKFPq4qBILBMXhYCEGiZRLZaWqgqgwAA5mxcSEJeUpdKWFT5ezJgVleq+XAHJ50NL6mKjbETTLzTS0py7ZwtO1nQaiSTGu7PXLverWUivZyY3S7TAoI9OMGucSGlCKWbI774zCSnG6QmebG84n46zqktcUg4FggXA6m6PbnqTEkGysIXZR3ooQ2Sry/365NBzFG5MVb9TL1+iwhkopgA/KZzPtglZ7TxExxWCFQ3uK8pIo9kepZa21+uNjfRQDdwESZvMnAf63T907G2l0peFjcQYbrUF5wFekTiK07T9C+MRPiE97Wi0bRwOEqoahQ1DZHAa6Nkib5OvW0x7geWBkFBxiblAAoETRACOdYNlm5IxKgDT1rhMIsIAAERAgANJyX7ZDChD1MRn6kSJCTTGQWBaKBfyBCCrCgY8WgCjqEBWJwoH1GYyYQJwADc2RiFiyygYQGIhDeTGiXUApwI5SBYAKwBsYQGhuWxcy6UCrRHHAABUcA0C53lAl57l+fpDBEn5nApIQwBWMAABeISeRFYgJUlKWYBl2Sue5CoEc2MIas6nCgFEILoFocAANoEQAun5UDSE1WXuW1zodU14U9ZhNC8VgAljkxa4SYRDbpBR9ZLDRQnRPWbpcXAo0CStHI9jhgnvrN0myfJemmP4SmmNklnWdkuRNnUhARVFPmzDFpgGQ2fl+HOEDoHUBG5fs+XpSEz2fVVeWpYVj0ldNzazX5qBIICqDLiwtKidOqq7VNmMxHUkw9lxxFeosmIiO1Yi9KYIQDpGODJqmrDLgA/AKf7SgcYiBajiPIyEqMQnj0QE7NMK4xycN1ET0lUYsd109SOAOugQ7eRz9QOmYtOk4zdzM3AbMa/53PgrzzpiOERDwDDqAUPUVm2DUdS+c6sUQOD0qW9bcuCsKMD20CN3Ie0rvSu7nv1N7xByyrFA7vaYjAJ4DXRLubpngi60noiTDEbu1ogWQCemFgtOGmG61QrLDjJ6nZUYfNVECqX5fMYU60hGurfPnnoFyaBSMo2jz5TfSAHDnnMSk/67Sk1qupsBzWs09P9N62mgtG5ZAVm0ooHR/Ai0NxPw1wGcqAQLIzZAxoLnAJgMANRAu5dyGZCnNAKHAlADjEDTmJOQhnbuUbOb9GRwEACmEMQe4ITgLAmMfcB71CWPVOAABJTwnghDvQYKBAA7bcD6ds3ZnX+MIS6JDpRqQ0lpdAOkgymXMn5R2IRwDyyiLee62QBTUUbI9aiDknIvj8g7XewVQo8L4UCXhAoNCiNCjQAAEvpFgABVJ2XolpWHogorEv95IEKIXFc20osIqPeuop2gtHgPUjC3MuCVoBQC0EAA)
+[Solution](https://live.lean-lang.org/#codez=JYWwDg9gTgLgBAWQIYwBYBtgCMB0AVJAYxmEICgyBaSuAMSghAC45UYYwBnJgeh8M45gEQjgCmYnmIDunATwBMABiUBOHgBMAnlgBWYqDxBJgAOwAKSdCE5jKUMQDdgtjTjAaAZhTMaArsTAjmJwAKIAHmBwABSAjcBwLHhaYGIAlGQAPnBIYFEsEVHxgEmEYZFwxaWFmXDAGnAJleXVYuhiIA0VBU1mnsDhDQCMKnAARHCAuNSjcAC8AHyVODlgFFQ0ACK1pgDk8BpihOhIDnBoIQDKYjAQtTWmnDBIpoQhntAnqC5wWpdkvgEkwTghAgpkcUAa0S6sVScBKkLK0NhcHMDGWWSQnE4IjgAG8QmItnACYT8giAL4NYGg8HRaIhSYEmEMrZbGF0iYxAkc4mpdJZWoAfVanngePqpMKFPq4qBILBMXhYCEGiZRLZaWqgqgwAA5mxcSEJeUpdKWFT5ezJgVleq+XAHJ50NL6mKjbETTLzTS0py7ZwtO1nQaiSTGu7PXLverWUivZyY3S7TAoI9OMGucSGlCKWbI774zCSnG6QmebG84n46zqktcUg4FggXA6m6PbnqTEkGysIXZR3ooQ2Sry/365NBzFG5MVb9TL1+iwhkopgA/KZzPtglZ7TxExxWCFQ3uK8pIo9kepZa21+uNjfRQDdwESZvMnAf63T907G2l0peFjcQYbrUF5wFekTiK07T9C+MRPiE97Wi0bRwOEqoahQ1DZHAa6Nkib5OvW0x7geWBkFBxiblAAoETRACOdYNlm5IxKgDT1rhMIsIAAERAgANJyX7ZDChD1MRn6kSJCTTGQWBaKBfyBCCrCgY8WgCjqEBWJwoH1GYyYQJwADc2RiFiyygYQGIhDeTGiXUApwI5SBYAKwBsYQGhuWxcy6UCrRHHAABUcA0C53lAl57l+fpDBEn5nApIQwBWMAABeISeRFYgJUlKWYBl2Sue5CoEc2MIas6nCgFEILoFocAANoEQAun5UDSE1WXuW1zodU14U9ZhNC8VgAljkxa4SYRDbpBR9ZLDRQnRPWbpcXAo0CStHI9jhgnvrN0myfJemmP4SmmNklnWdkuRNnUhARVFPmzDFpgGQ2fl+HOEDoHUBG5fs+XpSEz2fVVeWpYVj0ldNzazX5qBIICqDLiwtKidOqq7VNmMxHUkw9lxxFeosmIiO1Yi9KYIQDpGODJqmrDLgA/AKf7SgcYiBajiPIyEqMQnj0QE7NMK4xycN1ET0lUYsd109SOAOugQ7eRz9QOmYtOk4zdzM3AbMa/53PgrzzpiOERDwDDqAUPUVm2DUdS+c6sUQOD0qW9bcuCsKMD20CN3Ie0rvSu7nv1N7xByyrFA7vaYjAJ4DXRLubpngi60noiTDEbu1ogWQCemFgtOGmG61QrLDjJ6nZUYfNVECqX5fMYU60hGurfPnnoFyaBSMo2jz5TfSAHDnnMSk/67Sk1qupsBzWs09P9N62mgtG5ZAVm0ooHR/Ai0NxPw1wGcqAQLIzZAxoLnAJgMANRAu5dyGZCnNAKHAlADjEDTmJOQhnbuUbOb9GRwEACmEMQe4ITgLAmMfcB71CWPVOAABJTwnghDvQYKBAA7bcD6ds3ZnX+MIS6JDpRqQ0lpdAOkgymXMn5R2IRwDyyiLee62QBTUUbI9aiDknIvj8g7XewVQo8L4UCXhAoNCiNYPzbIAiBRYBbJ2DkE4ppTnKrLUmN5ZH8NkfIxhh9m60TEAxIghi6iF3kQQohcVzbSiHgLAYDQ36wL0ZGFuZd4p9SptrNeSsN6sHcdvZ0XMebuMptIbUMAQiNVRr1L2VsY6KzBL4/ErIcCzyAA)
 
 With `correctness` in place, Lean can now instantly decide any `a ~ b` problem through reflexivity, i.e.:
 
@@ -242,32 +257,21 @@ theorem example1'
         : (one.app two).app  ((zero.app zero).app three)
         ~ (one.app (two.app (three.app zero))) :=
   by
-  /- Try this:
-    exact (correctness ((one ⬝ two) ⬝ ((zero ⬝ zero) ⬝ three)) (one ⬝ (two ⬝ (three ⬝ zero)))).mpr rfl
-  -/
-  exact?
+  exact (correctness).mpr rfl
 
 -- (0 ⬝ (1 ⬝ 0)) ⬝ ((0 ⬝  2) ⬝ (3 ⬝ 0)) ~ 1 ⬝ (2 ⬝ (3 ⬝ 0))
 theorem example2'
   : (zero.app (one.app zero)).app ((zero.app two).app (three.app zero))
   ~ (one.app (two.app (three.app zero))) :=
   by
-  /- Try this:
-    exact (correctness ((zero ⬝ (one ⬝ zero)) ⬝ ((zero ⬝ two) ⬝ (three ⬝ zero)))
-      (one ⬝ (two ⬝ (three ⬝ zero)))).mpr rfl
-  -/
-  exact?
+  exact (correctness).mpr rfl
 
 -- (1 ⬝ 2) ⬝ ((0 ⬝ 0) ⬝ 3) ~ (0 ⬝ (1 ⬝ 0)) ⬝ ((0 ⬝  2) ⬝ (3 ⬝ 0))
 theorem example3'
   : (one.app two).app  ((zero.app zero).app three)
   ~ (zero.app (one.app zero)).app ((zero.app two).app (three.app zero)) :=
   by
-  /- Try this:
-    exact (correctness ((one ⬝ two) ⬝ ((zero ⬝ zero) ⬝ three))
-      ((zero ⬝ (one ⬝ zero)) ⬝ ((zero ⬝ two) ⬝ (three ⬝ zero)))).mpr rfl
-  -/
-  exact?
+  exact (correctness).mpr rfl
 ```
 # GodelT-Rewriting
 
@@ -312,8 +316,7 @@ inductive convrT : (ExpT α) → (ExpT α) → Prop
 | S     : convrT (S ⬝ x ⬝ y ⬝ z) (x ⬝ z ⬝ (y ⬝ z))
 | app   : convrT (a) (b) → convrT (c) (d) → convrT (a ⬝ c) (b ⬝ d)
 | recN_zero : convrT (recN ⬝ e ⬝ f ⬝ .zero) (e)
--- TO-DO: Fix Verso so it lets me define this constructor!!
---| recN_succ : convrT (recN ⬝ e ⬝ f ⬝ (.succ ⬝ n)) (f ⬝ n ⬝ (recN ⬝ e ⬝ f ⬝ n))
+| recN_succ : convrT (recN ⬝ e ⬝ f ⬝ (.succ ⬝ n)) (f ⬝ n ⬝ (recN ⬝ e ⬝ f ⬝ n))
 infix : 100 " ~ " => convrT
 ```
 Some rewriting examples are:
@@ -325,14 +328,10 @@ def I {β : Ty} : ExpT (α ⇒' α) := (@ExpT.S α (β ⇒' α) α) ⬝ .K ⬝ .
 example {x : ExpT α}
         : ((@I α β) ⬝ x)  ~  x :=
   by
-  /-
-  apply convrT.trans convrT.S ?_
-  apply convrT.trans convrT.K ?_
-  exact convrT.refl
-  -/
-  -- TO-DO: Try-it! Here
   sorry
 ```
+[Try it!](https://live.lean-lang.org/#codez=LTAEDECcHsFsC5QAsAuKAOBneB6HBjTAOgEtp8iBTSnSgd00JwCYAGVgThwBMBPAIwBWlSDlgBDEgDsACuIA2sTJWCRKANxLLuRdNwBmAKBKx00SClABZcSiTyS/IgBVx+FCXyHjU7gFd3EnVKUGdeUEQw9EpDAB9QADlbCNDeONBxSBg6FLDQQCTCVILUw2hoqRLpfRIAD0gUgEZ2UAAiUEAlwgByVtAAXgA+DKzoOm9pf0Dg0ABRGvRc8MKomPiAaVAAb3FQfgWAX1BDw8QZudAACm2unY7u8QBKdIBlTe3d/H2jk9n588vbm7XfD3AH/a78EHXMHdYGPeIAQXQ8y2N0ivAOx0OPwuV26EOK2O2hWx/HSAC8RNAjtSaSlTvMkih0pgAh9abTvmdzoyAYy4aA1PgEq9Pl8sVzcRceddJQ9eckZY8ypQKj8fNUavJGs02oBcah6A1AiPQ3h8Ew8U3w0Ck6nqiEABcCbQCNwPsADQXbFOkGFc6e72gGQwE3xNT6LUbF1ovYbEKIT17QzslJWm31c6UEHp/mYXiwI4R/Yx0CUbpxs5OhNJxAp20XDN1zr+mtpkuZjPpFCQcRSTDOwshEvFzql+mgCuJ9nV621rMNpvTluNhtLwrNutt4f89bUguAJuBCzUUvHNuEy/Nd5XJ6A1+d1vrD/reJmavyXjuXfvAM3AUY2h7PF0/AF92uL0Dg2U9R3OQDrl3e4wLJI8zk/S8OWvBcLhee9QEfbDQDJZ9cIQ/VznCfV8P5cQkXzD9PhRXZ/3OYDulAzYPm4RDzxQmkp1THFM3xVd0POYELm4edeP+fURPOXZ9TE9JBQSAB9CkYD7KNNljUcK02fQOKlBVmIBUCJ1Qm9FNwkJ9T0sjKTbflFKUll8A+AsNI2Cp/0ZMCtOPDY9IY6UjJAuDTO4tCJIs/UrNAGyLmcj59Ske5MziipiKi4tcLSlL1VqbVWB6AA/A1BmbbwQFAABJbgVQ8FBwgAYTgfhpFscxDFqvSqs2fcNIYl0QoiXoLgAAR+IgXhdRjjJBL1cKIO9QEW7xKBqcRTHkLS/lGnqPxBe8QVAErQD/XoJ34NJDkqgAJaQUHgCdKp6+8nrAPpQEw0AlqWmo3sOE7ftw29cJff7jtOidMHMSBeCAA)
+[Solution](https://live.lean-lang.org/#codez=LTAEDECcHsFsC5QAsAuKAOBneB6HBjTAOgEtp8iBTSnSgd00JwCYAGVgThwBMBPAIwBWlSDlgBDEgDsACuIA2sTJWCRKANxLLuRdNwBmAKBKx00SClABZcSiTyS/IgBVx+FCXyHjU7gFd3EnVKUGdeUEQw9EpDAB9QADlbCNDeONBxSBg6FLDQQCTCVILUw2hoqRLpfRIAD0gUgEZ2UAAiUEAlwgByVtAAXgA+DKzoOm9pf0Dg0ABRGvRc8MKomPiAaVAAb3FQfgWAX1BDw8QZudAACm2unY7u8QBKdIBlTe3d/H2jk9n588vbm7XfD3AH/a78EHXMHdYGPeIAQXQ8y2N0ivAOx0OPwuV26EOK2O2hWx/HSAC8RNAjtSaSlTvMkih0pgAh9abTvmdzoyAYy4aA1PgEq9Pl8sVzcRceddJQ9eckZY8ypQKj8fNUavJGs02oBcah6A1AiPQ3h8Ew8U3w0Ck6nqiEABcCbQCNwPsADQXbFOkGFc6e72gGQwE3xNT6LUbF1ovYbEKIT17QzslJWm31c6UEHp/mYXiwI4R/Yx0CUbpxs5OhNJxAp20XDN1zr+mtpkuZjPpFCQcRSTDOwshEvFzql+mgCuJ9nV621rMNpvTluNhtLwrNutt4f89bUguAJuBCzUUvHNuEy/Nd5XJ6A1+d1vrD/reJmavyXjuXfvAM3AUY2h7PF0/AF92uL0Dg2U9R3OQDrl3e4wLJI8zk/S8OWvBcLhee9QEfbDQDJZ9cIQ/VznCfV8P5cQkXzD9PhRXZ/3OYDulAzYPm4RDzxQmkp1THFM3xVd0POYELm4edeP+fURPOXZ9TE9JBQSAB9CkYD7KNNljUcK02fQOKlBVmIBUCJ1Qm9FNwkJ9T0sjKTbflFKUll8A+AsNI2Cp/0ZMCtOPDY9IY6UjJAuDTO4tCJIs/UrNAGyLmcj59Ske5MziipiKi4tcLSlL1VqbVWB6AA/A1BmbbwQFAABJbgVQ8FBwgAYTgfhpFscxDFqvSqs2fcNIYl0QoiXoLgAAR+IgXhdRjjJBL1cKIO9QEW7xKBqcRTHkLS/lGnqPxBe8QVAErQD/XoJ34NJDko9B5HCZsiE7btewel4AH4lInG67oi21Hq7HtfsgRbQA+ic1rcSwHtDeQgA)
 
 ```lean
 -- B Combinator
@@ -344,51 +343,60 @@ example {x : ExpT (b ⇒' c)}
         {z : ExpT a}
         : (B ⬝ x ⬝ y ⬝ z)  ~  (x ⬝ (y ⬝ z)) :=
   by
-  /-
-  unfold B
-  apply convrT.trans ?_ ?_
-  exact (.K ⬝ .S) ⬝ x ⬝ (.K ⬝ x) ⬝ y ⬝ z
-  · apply convrT.app ?_ convrT.refl
-    apply convrT.app ?_ convrT.refl
-    exact convrT.S
-  · apply convrT.trans ?_ ?_
-    exact .S ⬝ (.K ⬝ x) ⬝ y ⬝ z
-    · apply convrT.app ?_ convrT.refl
-      apply convrT.app ?_ convrT.refl
-      apply convrT.app ?_ convrT.refl
-      exact convrT.K
-    · apply convrT.trans ?_ ?_
-      exact (.K ⬝ x ⬝ z) ⬝ (y ⬝ z)
-      · exact convrT.S
-      · apply convrT.app ?_ convrT.refl
-        exact convrT.K
-  -/
-  -- TO-DO: Try-it! here
   sorry
 ```
+[Try it!](https://live.lean-lang.org/#codez=LTAEDECcHsFsC5QAsAuKAOBneB6HBjTAOgEtp8iBTSnSgd00JwCYAGVgThwBMBPAIwBWlSDlgBDEgDsACuIA2sTJWCRKANxLLuRdNwBmAKBKx00SClABZcSiTyS/IgBVx+FCXyHjU7gFd3EnVKUGdeUEQw9EpDAB9QADlbCNDeONBxSBg6FLDQQCTCVILUw2hoqRLpfRIAD0gUgEZ2UAAiUEAlwgByVtAAXgA+DKzoOm9pf0Dg0ABRGvRc8MKomPiAaVAAb3FQfgWAX1BDw8QZudAACm2unY7u8QBKdIBlTe3d/H2jk9n588vbm7XfD3AH/a78EHXMHdYGPeIAQXQ8y2N0ivAOx0OPwuV26EOK2O2hWx/HSAC8RNAjtSaSlTvMkih0pgAh9abTvmdzoyAYy4aA1PgEq9Pl8sVzcRceddJQ9eckZY8ypQKj8fNUavJGs02oBcah6A1AiPQ3h8Ew8U3w0Ck6nqiEABcCbQCNwPsADQXbFOkGFc6e72gGQwE3xNT6LUbF1ovYbEKIT17QzslJWm31c6UEHp/mYXiwI4R/Yx0CUbpxs5OhNJxAp20XDN1zr+mtpkuZjPpFCQcRSTDOwshEvFzql+mgCuJ9nV621rMNpvTluNhtLwrNutt4f89bUguAJuBCzUUvHNuEy/Nd5XJ6A1+d1vrD/reJmavyXjuXfvAM3AUY2h7PF0/AF92uL0Dg2U9R3OQDrl3e4wLJI8zk/S8OWvBcLhee9QEfbDQDJZ9cIQ/VznCfV8P5cQkXzD9PhRXZ/3OYDulAzYPm4RDzxQmkp1THFM3xVd0POYELm4edeP+fURPOXZ9TE9JBQSAB9CkYD7KNNljUcK02fQOKlBVmIBUCJ1Qm9FNwkJ9T0sjKTbflFKUll8A+AsNI2Cp/0ZMCtOPDY9IY6UjJAuDTO4tCJIs/UrNAGyLmcj59Ske5MziipiKi4tcLSlL1VqbVWB6AA/A1BmbbwQFAAAhUAAGE4H4aRbHMQxuEoPSaro69PgYmSAREqFJXxGV+pBeBelATCLjvSaQX1VZTUoGpxFMeQQl/fS+qBUKk3Azahp29kNgQ/9xC46lEHOGqsJwsiQVAEqLgfC5SLwlKIl6Cd+DSQ5KoACWkFB4AnSrrtAZ7XrJEGwAmqbb1wp45tAGaIcI6GHumhGkee+H7yRyH0ZKuGUfxtHfrAErcfBwikZImnCep4jIceQ5MHMSBeCAA)
+[Solution](https://live.lean-lang.org/#codez=LTAEDECcHsFsC5QAsAuKAOBneB6HBjTAOgEtp8iBTSnSgd00JwCYAGVgThwBMBPAIwBWlSDlgBDEgDsACuIA2sTJWCRKANxLLuRdNwBmAKBKx00SClABZcSiTyS/IgBVx+FCXyHjU7gFd3EnVKUGdeUEQw9EpDAB9QADlbCNDeONBxSBg6FLDQQCTCVILUw2hoqRLpfRIAD0gUgEZ2UAAiUEAlwgByVtAAXgA+DKzoOm9pf0Dg0ABRGvRc8MKomPiAaVAAb3FQfgWAX1BDw8QZudAACm2unY7u8QBKdIBlTe3d/H2jk9n588vbm7XfD3AH/a78EHXMHdYGPeIAQXQ8y2N0ivAOx0OPwuV26EOK2O2hWx/HSAC8RNAjtSaSlTvMkih0pgAh9abTvmdzoyAYy4aA1PgEq9Pl8sVzcRceddJQ9eckZY8ypQKj8fNUavJGs02oBcah6A1AiPQ3h8Ew8U3w0Ck6nqiEABcCbQCNwPsADQXbFOkGFc6e72gGQwE3xNT6LUbF1ovYbEKIT17QzslJWm31c6UEHp/mYXiwI4R/Yx0CUbpxs5OhNJxAp20XDN1zr+mtpkuZjPpFCQcRSTDOwshEvFzql+mgCuJ9nV621rMNpvTluNhtLwrNutt4f89bUguAJuBCzUUvHNuEy/Nd5XJ6A1+d1vrD/reJmavyXjuXfvAM3AUY2h7PF0/AF92uL0Dg2U9R3OQDrl3e4wLJI8zk/S8OWvBcLhee9QEfbDQDJZ9cIQ/VznCfV8P5cQkXzD9PhRXZ/3OYDulAzYPm4RDzxQmkp1THFM3xVd0POYELm4edeP+fURPOXZ9TE9JBQSAB9CkYD7KNNljUcK02fQOKlBVmIBUCJ1Qm9FNwkJ9T0sjKTbflFKUll8A+AsNI2Cp/0ZMCtOPDY9IY6UjJAuDTO4tCJIs/UrNAGyLmcj59Ske5MziipiKi4tcLSlL1VqbVWB6AA/A1BmbbwQFAAAhUAAGE4H4aRbHMQxuEoPSaro69PgYmSAREqFJXxGV+pBeBelATCLjvSaQX1VZTUoGpxFMeQQl/fS+qBUKk3Azahp29kNgQ/9xC46lEHOGqsJwsiQVAEqLgfC5SLwlKIl6Cd+DSQ4/CkfRoHkdiqonSj0HkcJmyITtu17AB+JTQARiclrcSxb1wp45tAZ6MfvbHXrJCcAHaMiRCGIttIgwaRxGodDeQwrBimoZphHKcgIgGbC1H3A5ognhJsnwchhdoa7Htadpnnlr5qa8ZxgnCLC0nmdF1Nqao9n6faxnaTV/m2bpsXuf18n1apo3+dNmlecsKGFupVXzf5mHJfZ5HaTt6bcOe/DcJIwjHlpUnvahwWQ+FlmxatnWwzC6kw7F1YgA)
+
 
 ```lean
-def add (m n : ExpT .Nat) := .recN ⬝ m ⬝ (.K ⬝ .succ) ⬝ n
+def add (m : ExpT .Nat) := .recN ⬝ m ⬝ (.K ⬝ .succ)
 
-example : (add m .zero)  ~  m :=
+-- m + 0 ~ m
+example : (add m ⬝ .zero)  ~  m :=
   by
-  /-
-  exact convrT.recN_zero
-  -/
-  -- TO-DO: "Try-it!" here
   sorry
 
-example : (add m (.succ ⬝ n))  ~  (.succ ⬝ (add m n)) :=
+-- m + (succ n) ~ succ (m + n)
+example : (add m ⬝ (.succ ⬝ n))  ~  (.succ ⬝ (add m ⬝ n)) :=
   by
-  /-
-  unfold add
-  apply convrT.trans ?_ ?_
-  exact (.K ⬝ .succ) ⬝ n ⬝ (.recN ⬝ m ⬝ (.K ⬝ .succ) ⬝ n)
-  · sorry --exact convrT.recN_succ
-  · apply convrT.app ?_ convrT.refl
-    exact convrT.K
-  -/
-  -- TO-DO: "Try-it!" here
+  sorry
+```
+[Try it!](https://live.lean-lang.org/#codez=LTAEDECcHsFsC5QAsAuKAOBneB6HBjTAOgEtp8iBTSnSgd00JwCYAGVgThwBMBPAIwBWlSDlgBDEgDsACuIA2sTJWCRKANxLLuRdNwBmAKBKx00SClABZcSiTyS/IgBVx+FCXyHjU7gFd3EnVKUGdeUEQw9EpDAB9QADlbCNDeONBxSBg6FLDQQCTCVILUw2hoqRLpfRIAD0gUgEZ2UAAiUEAlwgByVtAAXgA+DKzoOm9pf0Dg0ABRGvRc8MKomPiAaVAAb3FQfgWAX1BDw8QZudAACm2unY7u8QBKdIBlTe3d/H2jk9n588vbm7XfD3AH/a78EHXMHdYGPeIAQXQ8y2N0ivAOx0OPwuV26EOK2O2hWx/HSAC8RNAjtSaSlTvMkih0pgAh9abTvmdzoyAYy4aA1PgEq9Pl8sVzcRceddJQ9eckZY8ypQKj8fNUavJGs02oBcah6A1AiPQ3h8Ew8U3w0Ck6nqiEABcCbQCNwPsADQXbFOkGFc6e72gGQwE3xNT6LUbF1ovYbEKIT17QzslJWm31c6UEHp/mYXiwI4R/Yx0CUbpxs5OhNJxAp20XDN1zr+mtpkuZjPpFCQcRSTDOwshEvFzql+mgCuJ9nV621rMNpvTluNhtLwrNutt4f89bUguAJuBCzUUvHNuEy/Nd5XJ6A1+d1vrD/reJmavyXjuXfvAM3AUY2h7PF0/AF92uL0Dg2U9R3OQDrl3e4wLJI8zk/S8OWvBcLhee9QEfbDQDJZ9cIQ/VznCfV8P5cQkXzD9PhRXZ/3OYDulAzYPm4RDzxQmkp1THFM3xVd0POYELm4edeP+fURPOXZ9TE9JBQSAB9CkYD7KNNljUcK02fQOKlBVmIBUCJ1Qm9FNwkJ9T0sjKTbflFKUll8A+AsNI2Cp/0ZMCtOPDY9IY6UjJAuDTO4tCJIs/UrNAGyLmcj59Ske5MziipiKi4tcLSlL1VqbVWB6AA/A1BmbbxuEoPTxG4djzjzLzbBBeBegFSghVwvNiLvUAEseQwQFAPMAGpQEKkrYEMSganEUx5C0y5aqGwi7MOErlpaid+DSQ5BoACWkFBEAAIXCa0QmgPToD8eoLKK1Q/HmzAJ0wcxIDSAawBG+LWVAZLQBKhKLm+5KppmuaFpq9iup+lzcOSkEAcOc4geIqHlqSlKIl6LadtAfbDsQCdBvRmGUd+zHibAVrMrJnq+tw8m4cp3awBK29cIZpLGdpxn6dZEEWfx6mLn5lzBb+xnSfhx5WaR1GcSWmHQcOV6sl4IA)
+[Solution](https://live.lean-lang.org/#codez=LTAEDECcHsFsC5QAsAuKAOBneB6HBjTAOgEtp8iBTSnSgd00JwCYAGVgThwBMBPAIwBWlSDlgBDEgDsACuIA2sTJWCRKANxLLuRdNwBmAKBKx00SClABZcSiTyS/IgBVx+FCXyHjU7gFd3EnVKUGdeUEQw9EpDAB9QADlbCNDeONBxSBg6FLDQQCTCVILUw2hoqRLpfRIAD0gUgEZ2UAAiUEAlwgByVtAAXgA+DKzoOm9pf0Dg0ABRGvRc8MKomPiAaVAAb3FQfgWAX1BDw8QZudAACm2unY7u8QBKdIBlTe3d/H2jk9n588vbm7XfD3AH/a78EHXMHdYGPeIAQXQ8y2N0ivAOx0OPwuV26EOK2O2hWx/HSAC8RNAjtSaSlTvMkih0pgAh9abTvmdzoyAYy4aA1PgEq9Pl8sVzcRceddJQ9eckZY8ypQKj8fNUavJGs02oBcah6A1AiPQ3h8Ew8U3w0Ck6nqiEABcCbQCNwPsADQXbFOkGFc6e72gGQwE3xNT6LUbF1ovYbEKIT17QzslJWm31c6UEHp/mYXiwI4R/Yx0CUbpxs5OhNJxAp20XDN1zr+mtpkuZjPpFCQcRSTDOwshEvFzql+mgCuJ9nV621rMNpvTluNhtLwrNutt4f89bUguAJuBCzUUvHNuEy/Nd5XJ6A1+d1vrD/reJmavyXjuXfvAM3AUY2h7PF0/AF92uL0Dg2U9R3OQDrl3e4wLJI8zk/S8OWvBcLhee9QEfbDQDJZ9cIQ/VznCfV8P5cQkXzD9PhRXZ/3OYDulAzYPm4RDzxQmkp1THFM3xVd0POYELm4edeP+fURPOXZ9TE9JBQSAB9CkYD7KNNljUcK02fQOKlBVmIBUCJ1Qm9FNwkJ9T0sjKTbflFKUll8A+AsNI2Cp/0ZMCtOPDY9IY6UjJAuDTO4tCJIs/UrNAGyLmcj59Ske5MziipiKi4tcLSlL1VqbVWB6AA/A1BmbbxuEoPTxG4djzjzLzbBBeBegFSghVwvNiLvUAEseQwQFAPMAGpQEKkrYEMSganEUx5C0y5aqGwi7MOErlpaid+DSQ5prcSxmyIRzVOgU1BpG+LWVAZLQBKhKLgu5KppmuaFpq9iusulzcOSkFbsOc57uI97lqSlKIl6LadtAPwpH0aB5HY96J0o9B5HCQ7O27XsAH4lNAPGJz29wLh6vqftw85Ms+29cPJsGJwAduLGaScOxyEqZjIkXRiLbSIVGCfx9mqvkMLiYOhciFWIA)
+
+```lean
+def mult (m : ExpT .Nat) := .recN ⬝ .zero ⬝ (.K ⬝ (add m))
+
+-- m * 0 ~ 0
+example : (mult m ⬝ .zero) ~ .zero :=
+  by
+  sorry
+
+-- m * (succ n) ~ m + (m * n)
+example : (mult m ⬝ (.succ ⬝ n)) ~ ((add m) ⬝ (mult m ⬝ n)) :=
+  by
+  sorry
+```
+[Try it!](https://live.lean-lang.org/#codez=LTAEDECcHsFsC5QAsAuKAOBneB6HBjTAOgEtp8iBTSnSgd00JwCYAGVgThwBMBPAIwBWlSDlgBDEgDsACuIA2sTJWCRKANxLLuRdNwBmAKBKx00SClABZcSiTyS/IgBVx+FCXyHjU7gFd3EnVKUGdeUEQw9EpDAB9QADlbCNDeONBxSBg6FLDQQCTCVILUw2hoqRLpfRIAD0gUgEZ2UAAiUEAlwgByVtAAXgA+DKzoOm9pf0Dg0ABRGvRc8MKomPiAaVAAb3FQfgWAX1BDw8QZudAACm2unY7u8QBKdIBlTe3d/H2jk9n588vbm7XfD3AH/a78EHXMHdYGPeIAQXQ8y2N0ivAOx0OPwuV26EOK2O2hWx/HSAC8RNAjtSaSlTvMkih0pgAh9abTvmdzoyAYy4aA1PgEq9Pl8sVzcRceddJQ9eckZY8ypQKj8fNUavJGs02oBcah6A1AiPQ3h8Ew8U3w0Ck6nqiEABcCbQCNwPsADQXbFOkGFc6e72gGQwE3xNT6LUbF1ovYbEKIT17QzslJWm31c6UEHp/mYXiwI4R/Yx0CUbpxs5OhNJxAp20XDN1zr+mtpkuZjPpFCQcRSTDOwshEvFzql+mgCuJ9nV621rMNpvTluNhtLwrNutt4f89bUguAJuBCzUUvHNuEy/Nd5XJ6A1+d1vrD/reJmavyXjuXfvAM3AUY2h7PF0/AF92uL0Dg2U9R3OQDrl3e4wLJI8zk/S8OWvBcLhee9QEfbDQDJZ9cIQ/VznCfV8P5cQkXzD9PhRXZ/3OYDulAzYPm4RDzxQmkp1THFM3xVd0POYELm4edeP+fURPOXZ9TE9JBQSAB9CkYD7KNNljUcK02fQOKlBVmIBUCJ1Qm9FNwkJ9T0sjKTbflFKUll8A+AsNI2Cp/0ZMCtOPDY9IY6UjJAuDTO4tCJIs/UrNAGyLmcj59Ske5MziipiKi4tcLSlL1VqbVWB6AA/A1BmbbxuEoPTxG4djzjzLzbBBeBelAIhMrzYi71ABLHkMSq9NgPx5Eser9L5CJWsy1SqS63DLlq0BYFywwQCW0AACpQEKkrWEMSganEUx5C0+rhssTq8Ls0ASpmyaJ34NJDjWgAJaQUEQAAhcJrRCaA9OgPx6gsorVGGyhMAnTBzEgNJVrAPMtvOBLQGSm71oAaguRHUceA6jvQE6UjOkb1uIlGkpS9G/hq9jlvmobScu5Lmt6B6ntAV73sQCc1sZi75op3HebAKbKCFQjKXm7qFrpqnydZXDkpF6mZdppb5dR+bpqlubiPV5aQUplXWtveaDc19LsfOsnheesAStljWGZt5nHkOaGsl4IA)
+[Solution](https://live.lean-lang.org/#codez=LTAEDECcHsFsC5QAsAuKAOBneB6HBjTAOgEtp8iBTSnSgd00JwCYAGVgThwBMBPAIwBWlSDlgBDEgDsACuIA2sTJWCRKANxLLuRdNwBmAKBKx00SClABZcSiTyS/IgBVx+FCXyHjU7gFd3EnVKUGdeUEQw9EpDAB9QADlbCNDeONBxSBg6FLDQQCTCVILUw2hoqRLpfRIAD0gUgEZ2UAAiUEAlwgByVtAAXgA+DKzoOm9pf0Dg0ABRGvRc8MKomPiAaVAAb3FQfgWAX1BDw8QZudAACm2unY7u8QBKdIBlTe3d/H2jk9n588vbm7XfD3AH/a78EHXMHdYGPeIAQXQ8y2N0ivAOx0OPwuV26EOK2O2hWx/HSAC8RNAjtSaSlTvMkih0pgAh9abTvmdzoyAYy4aA1PgEq9Pl8sVzcRceddJQ9eckZY8ypQKj8fNUavJGs02oBcah6A1AiPQ3h8Ew8U3w0Ck6nqiEABcCbQCNwPsADQXbFOkGFc6e72gGQwE3xNT6LUbF1ovYbEKIT17QzslJWm31c6UEHp/mYXiwI4R/Yx0CUbpxs5OhNJxAp20XDN1zr+mtpkuZjPpFCQcRSTDOwshEvFzql+mgCuJ9nV621rMNpvTluNhtLwrNutt4f89bUguAJuBCzUUvHNuEy/Nd5XJ6A1+d1vrD/reJmavyXjuXfvAM3AUY2h7PF0/AF92uL0Dg2U9R3OQDrl3e4wLJI8zk/S8OWvBcLhee9QEfbDQDJZ9cIQ/VznCfV8P5cQkXzD9PhRXZ/3OYDulAzYPm4RDzxQmkp1THFM3xVd0POYELm4edeP+fURPOXZ9TE9JBQSAB9CkYD7KNNljUcK02fQOKlBVmIBUCJ1Qm9FNwkJ9T0sjKTbflFKUll8A+AsNI2Cp/0ZMCtOPDY9IY6UjJAuDTO4tCJIs/UrNAGyLmcj59Ske5MziipiKi4tcLSlL1VqbVWB6AA/A1BmbbxuEoPTxG4djzjzLzbBBeBelAIhMrzYi71ABLHkMSq9NgPx5Eser9L5CJWsy1SqS63DLlq0BYFywwQCW0AACpQEKkrWEMSganEUx5C0+rhssTq8Ls0ASpmyaJ34NJDgOtxLGbdrKCFFTKW8Na8y284EtAZKbvWgBqC5/uBx4XuO06hpG9biKBpKUtBv4avY5b5oRi7cOS5regep7QD8KR9GgeQsfOidKPQeRwneztu17AB+JTQHZicXvcC5uoWrG0aS+bpspeb+cxpahehicAHbi0O3n3schK5YyJEGYi20iDpzmOeVqr5DCnm3oXIhViAA)
+
+```lean
+def power (m : ExpT .Nat) := .recN ⬝ (.succ ⬝ .zero) ⬝ (.K ⬝ (mult m))
+
+-- m ^ 0 ~ 1
+example : (power m ⬝ .zero) ~ (.succ ⬝ .zero) :=
+  by
+  sorry
+
+-- m ^ (succ n) ~ m * (m ^ n)
+example : (power m ⬝ (.succ ⬝ n)) ~ ((mult m) ⬝ (power m ⬝ n)) :=
+  by
+  sorry
+
+-- m ^ 3 ~ m * (m * m)
+example : (power m ⬝ (.succ ⬝ (.succ ⬝  (.succ ⬝ .zero))))  ~  (mult m ⬝ (mult m ⬝ m)) :=
+  by
   sorry
 ```
 
@@ -443,20 +451,21 @@ Defining reification in this instance is simple because of how we evaluate types
 
 This give us the following reification function:
 ```lean
+def numeral : Nat → ExpT Ty.Nat
+| 0 => .zero
+| n+1 => .succ ⬝ (numeral n)
+
+
 def reifyT (a : Ty) (e : Ty_inter a) : ExpT a :=
 /-
-| Ty.Nat, (0 : ℕ) => zero
-| Ty.Nat, n+1     => succ ⬝ (reify Ty.Nat n)
+| Ty.Nat, e            => numeral e
 
-| Ty.arrow a b, (f, F) => f
+| Ty.arrow a b, (c, f) => c
 -/
 by
   cases a
-  case Nat =>
-    induction e
-    case zero           => exact .zero
-    case succ n reify_n => exact (.succ ⬝ reify_n)
-  case arrow a b        => exact e.fst
+  case Nat        => exact numeral e
+  case arrow a b  => exact e.fst
 ```
 In addition, we will need to define application on the Meta-level where our glued-on function `F : (Ty_inter a → Ty_inter b)`
 comes into play:
@@ -477,7 +486,7 @@ For a generic function `f : ExpT (α =>' β)`, we are going to keep applying `f`
 `f ⬝ (reify x1) ⬝ ... ⬝ (reify xn)` is fully-applied, then we will use `f`'s standard-translation on `x1, ..., xn`. This will in-effect
 capture all of `f`'s `~`-behavior into one big tuple which is how `F : Ty_inter a → Ty_inter b` works.
 
-We illustrate this with the exampe ` S :  ExpT ((a ⇒' b ⇒' c) ⇒' (a ⇒' b) ⇒' (a ⇒' c))`.
+We illustrate this with the example `S :  ExpT ((a ⇒' b ⇒' c) ⇒' (a ⇒' b) ⇒' (a ⇒' c))`.
 
 The first step is to evalute `S`'s type to the Meta-level, for readibility let:
 
@@ -539,10 +548,6 @@ def ExpT_inter (a : Ty) : (e : ExpT a) → Ty_inter a
               (λ z ↦ appsem (appsem x z) (appsem y z)))))))
 | @ExpT.App a b f e  => appsem (ExpT_inter (a ⇒' b) f) (ExpT_inter a e)
 
-| _ => sorry
-
--- TO-DO: Fix Verso so I can implement the rest of this Definition!!
-/-
 | ExpT.zero          => (0 : Nat)
 
 | ExpT.succ          => (.succ,
@@ -551,7 +556,218 @@ def ExpT_inter (a : Ty) : (e : ExpT a) → Ty_inter a
                    (λ p ↦ (.recN ⬝ (reifyT a p),
                    (λ q ↦ (.recN ⬝ (reifyT a p) ⬝ (reifyT (.Nat⇒'a⇒'a) q),
                    (λ n0 ↦ Nat.rec p (λ n r ↦ appsem (appsem q n) r) n0))))))
--/
+```
+
+As before with Monoid-Rewriting, we have that rewritable-terms give us equal evaluations:
+```lean
+theorem convrT_eval_eq {a : Ty} {e e' : ExpT a} : e ~ e' → ((ExpT_inter a e) = (ExpT_inter a e')) :=
+  by
+  -- Hint: Induction on convrT
+  sorry
+```
+[Try it!](https://live.lean-lang.org/#codez=LTAEDECcHsFsC5QAsAuKAOBneB6HBjTAOgEtp8iBTSnSgd00JwCYAGVgThwBMBPAIwBWlSDlgBDEgDsACuIA2sTJWCRKANxLLuRdNwBmAKBKx00SClABZcSiTyS/IgBVx+FCXyHjU7gFd3EnVKUGdeUEQw9EpDAB9QADlbCNDeONBxSBg6FLDQQCTCVILUw2hoqRLpfRIAD0gUgEZ2UAAiUEAlwgByVtAAXgA+DKzoOm9pf0Dg0ABRGvRc8MKomPiAaVAAb3FQfgWAX1BDw8QZudAACm2unY7u8QBKdIBlTe3d/H2jk9n588vbm7XfD3AH/a78EHXMHdYGPeIAQXQ8y2N0ivAOx0OPwuV26EOK2O2hWx/HSAC8RNAjtSaSlTvMkih0pgAh9abTvmdzoyAYy4aA1PgEq9Pl8sVzcRceddJQ9eckZY8ypQKj8fNUavJGs02oBcah6A1AiPQ3h8Ew8U3w0Ck6nqiEABcCbQCNwPsADQXbFOkGFc6e72gGQwE3xNT6LUbF1ovYbEKIT17QzslJWm31c6UEHp/mYXiwI4R/Yx0CUbpxs5OhNJxAp20XDN1zr+mtpkuZjPpFCQcRSTDOwshEvFzql+mgCuJ9nV621rMNpvTluNhtLwrNutt4f89bUguAJuBCzUUvHNuEy/Nd5XJ6A1+d1vrD/reJmavyXjuXfvAM3AUY2h7PF0/AF92uL0Dg2U9R3OQDrl3e4wLJI8zk/S8OWvBcLhee9QEfbDQDJZ9cIQ/VznCfV8P5cQkXzD9PhRXZ/3OYDulAzYPm4RDzxQmkp1THFM3xVd0POYELm4edeP+fURPOXZ9TE9JBQSAB9CkYD7KNNljUcK02fQOKlBVmIBUCJ1Qm9FNwkJ9T0sjKTbflFKUll8A+AsNI2Cp/0ZMCtOPDY9IY6UjJAuDTO4tCJIs/UrNAGyLmcj59Ske5MziipiKi4tcLSlL1VqbVWB6AA/A1BmbU1uEoPSwiU6QUBEBZimWdIwiIHlDUAVEJvHiTJsgyG5DWxaEdhBAB1i4arqhqiVSWqpHq+oIQqqqMiRZQ8zoz5zksNE5oWnEAQhDcFj26aQV2qbFoiXoLhQIhMF8IdHkMSq9LUEh9HCf40TbE7Loyc7R22eBekMHBgBa3g2tsd1zkKxAOpBQ1VOgSHoZQd0pAAagaGlDQS3Dznez7UnR0Bku60nepGfr+Fh/B3X0JGysMYAcEMfg0kOfBxGUXtxAnHnlESZIBjC8YAg8a1izCoWQhRpMjkNSgajcSwUdl3mQgJipid4JSKmV1X3Hi1lcL1g3Hm5rWhj6t4kyNtXiyIfRMCZbxXvpU602B1JAfTfS5SWfX/oF+IAAF1ntw1b1dMKk3OQBu4FAeZADLCC47wuPX+vQe448Vo4k9AABHUB09zlL+XDl57Y+GOnnzgvC+Tw90/OTCs8oD6vvELp+C6ESX0bpuLmT8I247omu5Jy4+4HkEX0J7PZ86fEn2Hpui4Q9PKKwSg80uNb99AQ98JxI+83CcjK9yiPjVp2Ksr6QZd/Wj05m9g7wRBJn3/QT/tjtniArRWMd4agERsyM2oDBjnAShvEezdyYpA6mXcmOMQRVwstsWkMdFIIMQaPFOaCp5CiXtPcI2xc4EMQUXUubdMpT27jnEEGUKEGRQF0XunQ5TFzzvHQhRcpCFXToyIggpiFCIFGg1+x9D57zzKXZKAoQTCJvrlD2K0pD8BCN9P2dZA7+0JOdG62dti+g/qHYsz1WZgBCCVQcoATDoAcJQXsABtdxlAAC63jtg3U8SWXxAt5D7wkBFW0SkNAKCiaXFE7kBwjkJAcRA9ihzFD+D8AB1i+h/2ya2ExHMuZOPmmpJAE4JaBGluUw4Ch5BKQAObQAUL2fAoTMj9USaAbw1thahi1C6EIYtqQgFAAASVgLASg3ASC2BiNSTA5hIBpEFjbHMeYXT23EEpSASldjiH4LVJAz8wqjImVMmZczYowDzAco5YVFlZBWb0kInZuy9k2TcD42zdm7EObs75hySDHP4PgI5JyRlgHOdM2Z9VrlwAyECkFYLgUPKWc868Nt1g0UPOEYZRxRkAAk6rwFOWATxmcHygF4L4slhwbqyLzBS3CNRfGgE8TS7xdLcmMvPgo9l7jVhss8ay7xIIBWcu5Qyi+FxR5p1AIAC/JM7Z3QO6UAid6Ep0AJfkIIRVsvFRy2lkL6WrX5Uq827C9XeLVRqtBVqtWHENVy41uSk6aqtbq9xkqXUBK9Uao4jzlk9MxcLF4NFAK4rwhCglYBiXzUQHSzxHcqWkTwv6w4oyeUyqTSy3CnKBVknTaATN0r+XyLfjm+8wq/VioLUWktpq37lrkbypN1bRWes5Z6wtzqY0mt5c2vM3KR4Ko7tnK17ph0j0TuPRVk9x3uI7eQ5hTq87dJdYgxO29G0tplafTMvKr73C1Q6slU6C6rrrb2jNYAs1mvnZaxdvjWGdxXTWtd572RbpkTKwdJ88IHplUerVn7aSgepJ4ntUqd0H15fuvlb8j3QYHXBgDErCL1tvaWiti6MPePQ2RTDJrPH/rIoTVNZ8i2BuKas4Wu8xygH3LXUA7Efl7OvDspSrGkXXm4OC/FN7QBxpQIgcA0B5DyBGL2EwFzYWUHkMUwT+gbmgAACIrWgHpLJ/0MiPURUc90+A+OooWei4NcsBSUCFCpSkDGEJ6QE8W2NJLE3uMykRR+tkYBEbvTh9z2Vq0ox89h3d/LPHuerfoZ9oBWDId/Sh7NbmrMJEC9FzxUXa2xZ9TBhDx9wO0gVYwhdPaP0bunSXNBhXkvLpJpB6LbDmF8MnWVpuydhFoLERIur+GpH1B3vFmVSiQSQFUawE966+2IPyzSdL0WYtxbNUVx9JWavhFm2K5rk2C5tZESLO6XX3E9qIbrH9ZbW3uIy+TYbo3T0tcVtN+b2XOtWavcd6R/WzuJcu8okbj3Ju+qg6Zp5E5aMhEcgTF0FR7PRsE8J0lxrwvVbI9ZQmBMkr3GCzlxHZDkexWrWj8mmPzv+esmyv9niEpsoptl4nSOo2k5654qQviMELabbTnHab8PrczEzlnDQrb/Zy3+8nSWhSpdrTzi4fPvGs5pwN/lD2jhVc50w2rh3n2bcE4Q5OmqVfCga+rlbhvwhNYm9rzd5NdvPY+N1t7fXhe8qGyoq342leHHdwKjL4rzgy7l0L3l+vVtXpfWrtbF3Nfm6c+V9rojbDiJe3b3rp32dfap9d13UfM0jwe779xzPZcC+gzb17yePup7CxH/DP3ef5/54L7XN0y+O7T9XjPMuOEJ9txrnrbX3st8r999vdexVs9Czhy7MvMwl6T33h3CXB/p5d1Ps9xr4S+FX329LuF0qd05x5nKROvs7+rSTzzhPr3R988fbfSUycc4N/TvH3OR8N+j0QD/Y+mUXZPz1mfPf7cU9x8b8q8rtl9X8v9ctv9J9X9O8Dsjtm8F8J8l9fsV8gdlkgA)
+[Solution](https://live.lean-lang.org/#codez=LTAEDECcHsFsC5QAsAuKAOBneB6HBjTAOgEtp8iBTSnSgd00JwCYAGVgThwBMBPAIwBWlSDlgBDEgDsACuIA2sTJWCRKANxLLuRdNwBmAKBKx00SClABZcSiTyS/IgBVx+FCXyHjU7gFd3EnVKUGdeUEQw9EpDAB9QADlbCNDeONBxSBg6FLDQQCTCVILUw2hoqRLpfRIAD0gUgEZ2UAAiUEAlwgByVtAAXgA+DKzoOm9pf0Dg0ABRGvRc8MKomPiAaVAAb3FQfgWAX1BDw8QZudAACm2unY7u8QBKdIBlTe3d/H2jk9n588vbm7XfD3AH/a78EHXMHdYGPeIAQXQ8y2N0ivAOx0OPwuV26EOK2O2hWx/HSAC8RNAjtSaSlTvMkih0pgAh9abTvmdzoyAYy4aA1PgEq9Pl8sVzcRceddJQ9eckZY8ypQKj8fNUavJGs02oBcah6A1AiPQ3h8Ew8U3w0Ck6nqiEABcCbQCNwPsADQXbFOkGFc6e72gGQwE3xNT6LUbF1ovYbEKIT17QzslJWm31c6UEHp/mYXiwI4R/Yx0CUbpxs5OhNJxAp20XDN1zr+mtpkuZjPpFCQcRSTDOwshEvFzql+mgCuJ9nV621rMNpvTluNhtLwrNutt4f89bUguAJuBCzUUvHNuEy/Nd5XJ6A1+d1vrD/reJmavyXjuXfvAM3AUY2h7PF0/AF92uL0Dg2U9R3OQDrl3e4wLJI8zk/S8OWvBcLhee9QEfbDQDJZ9cIQ/VznCfV8P5cQkXzD9PhRXZ/3OYDulAzYPm4RDzxQmkp1THFM3xVd0POYELm4edeP+fURPOXZ9TE9JBQSAB9CkYD7KNNljUcK02fQOKlBVmIBUCJ1Qm9FNwkJ9T0sjKTbflFKUll8A+AsNI2Cp/0ZMCtOPDY9IY6UjJAuDTO4tCJIs/UrNAGyLmcj59Ske5MziipiKi4tcLSlL1VqbVWB6AA/A1BmbU1uEoPSwiU6QUBEBZimWdIwiIHlDUAVEJvHiTJsgyG5DWxaEdhBAB1i4arqhqiVSWqpHq+oIQqqqMiRZQ8zoz5zksNE5oWnEAQhDcFj26aQV2qbFoiXoLhQIhMF8IdHkMSq9LUEh9HCf40TbE7Loyc7R22eBekMHBgBa3g2tsd1zkKxAOpBQ1VOgSHoZQd0pAAagaGlDQS3Dznez7UnR0Bku60nepGfr+Fh/B3X0JGysMYAcEMfg0kOfBxGUXtxAnHnlESZIBjC8YAg8a1izCoWQhRpMjkNSgajcSwUdl3mQgJipid4JSKmV1X3Hi1lcL1g3Hm5rWhj6t4kyNtXiyIfRMCZbxXvpU602B1JAfTfS5SWfX/oF+IAAF1ntw1b1dMKk3OQBu4FAeZADLCC47wuPX+vQe448Vo4k9AABHUB09zlL+XDl57Y+GOnnzgvC+Tw90/OTCs8oD6vvELp+C6ESX0bpuLmT8I247omu5Jy4+4HkEX0J7PZ86fEn2Hpui4Q9PKKwSg80uNb99AQ98JxI+83CcjK9yiPjVp2Ksr6QZd/Wj05m9g7wRBJn3/QT/tjtniArRWMd4agERsyM2oDBjnAShvEezdyYpA6mXcmOMQRVwstsWkMdFIIMQaPFOaCp5CiXtPcI2xc4EMQUXUubdMpT27jnEEGUKEGRQF0XunQ5TFzzvHQhRcpCFXToyIggpiFCIFGg1+x9D57zzKXZKAoQTCJvrlD2K0pD8BCN9P2dZA7+0JOdG62dti+g/qHYsz1WZgBCCVQcoATDoAcJQXsABtdxlAAC63jtg3U8SWXxAt5D7wkBFW0SkNAKCiaXFE7kBwjkJAcRA9ihzFD+D8AB1i+h/2ya2ExHMuZOPmmpJAE4JaBGluUw4Ch5BKQAObQAUL2fAoTMj9USaAbw1thahi1C6EIYtqSQDDD068Nscx5hdPbcQSlIBKV2OIfgtUkDPzCpAHI7jlmrO8eMuWoBOzdl7DMm4Hw5kLN2CshZ5yVkkDWfwfAqz1kjK2Ts+57pHm7P2TbdYNFDzhGGUcUZ8gfnCxeDRQCAK8IvOBWMw4gsba7zHKAfctdQDsQuYs688ylKYruWs/A3BnlAsOH4KQ+hoDyHYlky6Gy3kEvdES75iK+mUCFCpSkKKEJ6VJQKeF3TekhEcgTF0FQeWwsOCCoAA)
+
+
+## Nbe
+We now define NbE as before, we first evaluate the Term to the Meta-level before reifying the
+normalized term back down to the Object-level:
+
+```lean
+def nbeT (a : Ty) (e : ExpT a) : (ExpT a) := reifyT a (ExpT_inter a e)
+```
+
+Note that from `convrT_eval_eq` we immediately get soundness for our NbE algorithm:
+
+```lean
+theorem soundness {e e' : ExpT α} : e ~ e' → nbeT α e = nbeT α e' :=
+  by
+  -- Hint: Immediate from convrT_eval_eq
+  sorry
+```
+[Try it!](https://live.lean-lang.org/#codez=LTAEDECcHsFsC5QAsAuKAOBneB6HBjTAOgEtp8iBTSnSgd00JwCYAGVgThwBMBPAIwBWlSDlgBDEgDsACuIA2sTJWCRKANxLLuRdNwBmAKBKx00SClABZcSiTyS/IgBVx+FCXyHjU7gFd3EnVKUGdeUEQw9EpDAB9QADlbCNDeONBxSBg6FLDQQCTCVILUw2hoqRLpfRIAD0gUgEZ2UAAiUEAlwgByVtAAXgA+DKzoOm9pf0Dg0ABRGvRc8MKomPiAaVAAb3FQfgWAX1BDw8QZudAACm2unY7u8QBKdIBlTe3d/H2jk9n588vbm7XfD3AH/a78EHXMHdYGPeIAQXQ8y2N0ivAOx0OPwuV26EOK2O2hWx/HSAC8RNAjtSaSlTvMkih0pgAh9abTvmdzoyAYy4aA1PgEq9Pl8sVzcRceddJQ9eckZY8ypQKj8fNUavJGs02oBcah6A1AiPQ3h8Ew8U3w0Ck6nqiEABcCbQCNwPsADQXbFOkGFc6e72gGQwE3xNT6LUbF1ovYbEKIT17QzslJWm31c6UEHp/mYXiwI4R/Yx0CUbpxs5OhNJxAp20XDN1zr+mtpkuZjPpFCQcRSTDOwshEvFzql+mgCuJ9nV621rMNpvTluNhtLwrNutt4f89bUguAJuBCzUUvHNuEy/Nd5XJ6A1+d1vrD/reJmavyXjuXfvAM3AUY2h7PF0/AF92uL0Dg2U9R3OQDrl3e4wLJI8zk/S8OWvBcLhee9QEfbDQDJZ9cIQ/VznCfV8P5cQkXzD9PhRXZ/3OYDulAzYPm4RDzxQmkp1THFM3xVd0POYELm4edeP+fURPOXZ9TE9JBQSAB9CkYD7KNNljUcK02fQOKlBVmIBUCJ1Qm9FNwkJ9T0sjKTbflFKUll8A+AsNI2Cp/0ZMCtOPDY9IY6UjJAuDTO4tCJIs/UrNAGyLmcj59Ske5MziipiKi4tcLSlL1VqbVWB6AA/A1BmbU1uEoPSwiU6QUBEBZimWdIwiIHlDUAVEJvHiTJsgyG5DWxaEdhBAB1i4arqhqiVSWqpHq+oIQqqqMiRZQ8zoz5zksNE5oWnEAQhDcFj26aQV2qbFoiXoLhQIhMF8IdHkMSq9LUEh9HCf40TbE7Loyc7R22eBekMHBgBa3g2tsd1zkKxAOpBQ1VOgSHoZQd0pAAagaGlDQS3Dznez7UnR0Bku60nepGfr+Fh/B3X0JGysMYAcEMfg0kOfBxGUXtxAnHnlESZIBjC8YAg8a1izCoWQhRpMjkNSgajcSwUdl3mQgJipid4JSKmV1X3Hi1lcL1g3Hm5rWhj6t4kyNtXiyIfRMCZbxXvpU602B1JAfTfS5SWfX/oF+IAAF1ntw1b1dMKk3OQBu4FAeZADLCC47wuPX+vQe448Vo4k9AABHUB09zlL+XDl57Y+GOnnzgvC+Tw90/OTCs8oD6vvELp+C6ESX0bpuLmT8I247omu5Jy4+4HkEX0J7PZ86fEn2Hpui4Q9PKKwSg80uNb99AQ98JxI+83CcjK9yiPjVp2Ksr6QZd/Wj05m9g7wRBJn3/QT/tjtniArRWMd4agERsyM2oDBjnAShvEezdyYpA6mXcmOMQRVwstsWkMdFIIMQaPFOaCp5CiXtPcI2xc4EMQUXUubdMpT27jnEEGUKEGRQF0XunQ5TFzzvHQhRcpCFXToyIggpiFCIFGg1+x9D57zzKXZKAoQTCJvrlD2K0pD8BCN9P2dZA7+0JOdG62dti+g/qHYsz1WZgBCCVQcoATDoAcJQXsABtdxlAAC63jtg3U8SWXxAt5D7wkBFW0SkNAKCiaXFE7kBwjkJAcRA9ihzFD+D8AB1i+h/2ya2ExHMuZOPmmpJAE4JaBGluUw4Ch5BKQAObQAUL2fAoTMj9USaACc3Z9ZNJaRkNxZRBY213mOUA+5a6gHYuIJSkAlLvDmUpGZ/BapIGvNwNZz8wp+CkPoaA8h2JZMumFSAOR3HiFWSQJA7p8CbOud47wIAsoOO6E40wrjezaJCIA3J3zOmdEMKE2A4TMDQF2dwKQbjezxNSD5dJ/5xApJeekwo/zfk3XRQi0GhxOYThAAACTqogAAkiCyg3ASC2BCJzCJ8zon1MoKXCcYKsi8CAA)
+[Solution](https://live.lean-lang.org/#codez=LTAEDECcHsFsC5QAsAuKAOBneB6HBjTAOgEtp8iBTSnSgd00JwCYAGVgThwBMBPAIwBWlSDlgBDEgDsACuIA2sTJWCRKANxLLuRdNwBmAKBKx00SClABZcSiTyS/IgBVx+FCXyHjU7gFd3EnVKUGdeUEQw9EpDAB9QADlbCNDeONBxSBg6FLDQQCTCVILUw2hoqRLpfRIAD0gUgEZ2UAAiUEAlwgByVtAAXgA+DKzoOm9pf0Dg0ABRGvRc8MKomPiAaVAAb3FQfgWAX1BDw8QZudAACm2unY7u8QBKdIBlTe3d/H2jk9n588vbm7XfD3AH/a78EHXMHdYGPeIAQXQ8y2N0ivAOx0OPwuV26EOK2O2hWx/HSAC8RNAjtSaSlTvMkih0pgAh9abTvmdzoyAYy4aA1PgEq9Pl8sVzcRceddJQ9eckZY8ypQKj8fNUavJGs02oBcah6A1AiPQ3h8Ew8U3w0Ck6nqiEABcCbQCNwPsADQXbFOkGFc6e72gGQwE3xNT6LUbF1ovYbEKIT17QzslJWm31c6UEHp/mYXiwI4R/Yx0CUbpxs5OhNJxAp20XDN1zr+mtpkuZjPpFCQcRSTDOwshEvFzql+mgCuJ9nV621rMNpvTluNhtLwrNutt4f89bUguAJuBCzUUvHNuEy/Nd5XJ6A1+d1vrD/reJmavyXjuXfvAM3AUY2h7PF0/AF92uL0Dg2U9R3OQDrl3e4wLJI8zk/S8OWvBcLhee9QEfbDQDJZ9cIQ/VznCfV8P5cQkXzD9PhRXZ/3OYDulAzYPm4RDzxQmkp1THFM3xVd0POYELm4edeP+fURPOXZ9TE9JBQSAB9CkYD7KNNljUcK02fQOKlBVmIBUCJ1Qm9FNwkJ9T0sjKTbflFKUll8A+AsNI2Cp/0ZMCtOPDY9IY6UjJAuDTO4tCJIs/UrNAGyLmcj59Ske5MziipiKi4tcLSlL1VqbVWB6AA/A1BmbU1uEoPSwiU6QUBEBZimWdIwiIHlDUAVEJvHiTJsgyG5DWxaEdhBAB1i4arqhqiVSWqpHq+oIQqqqMiRZQ8zoz5zksNE5oWnEAQhDcFj26aQV2qbFoiXoLhQIhMF8IdHkMSq9LUEh9HCf40TbE7Loyc7R22eBekMHBgBa3g2tsd1zkKxAOpBQ1VOgSHoZQd0pAAagaGlDQS3Dznez7UnR0Bku60nepGfr+Fh/B3X0JGysMYAcEMfg0kOfBxGUXtxAnHnlESZIBjC8YAg8a1izCoWQhRpMjkNSgajcSwUdl3mQgJipid4JSKmV1X3Hi1lcL1g3Hm5rWhj6t4kyNtXiyIfRMCZbxXvpU602B1JAfTfS5SWfX/oF+IAAF1ntw1b1dMKk3OQBu4FAeZADLCC47wuPX+vQe448Vo4k9AABHUB09zlL+XDl57Y+GOnnzgvC+Tw90/OTCs8oD6vvELp+C6ESX0bpuLmT8I247omu5Jy4+4HkEX0J7PZ86fEn2Hpui4Q9PKKwSg80uNb99AQ98JxI+83CcjK9yiPjVp2Ksr6QZd/Wj05m9g7wRBJn3/QT/tjtniArRWMd4agERsyM2oDBjnAShvEezdyYpA6mXcmOMQRVwstsWkMdFIIMQaPFOaCp5CiXtPcI2xc4EMQUXUubdMpT27jnEEGUKEGRQF0XunQ5TFzzvHQhRcpCFXToyIggpiFCIFGg1+x9D57zzKXZKAoQTCJvrlD2K0pD8BCN9P2dZA7+0JOdG62dti+g/qHYsz1WZgBCCVQcoATDoAcJQXsABtdxlAAC63jtg3U8SWXxAt5D7wkBFW0SkNAKCiaXFE7kBwjkJAcRA9ihzFD+D8AB1i+h/2ya2ExHMuZOPmmpJAE4JaBGluUw4Ch5BKQAObQAUL2fAoTMj9USaACc3Z9ZNJaRkNxZRBY213mOUA+5a6gHYuIJSkAlLvDmUpGZ/BapIGvNwNZz8wp+CkPoaA8h2JZMumFSAOR3HiFWSQJA7p8CbOud47wIAsoOO6E40wrjezaJCIA3J3zOmdEMKE2A4TMDQF2dwKQbjezxNSD5dJ/5xApJeekwo/zfk3XRQi0GhxOYTl2fsw55MdEVNKVSJADQJxIHEFMJAzAOL5Nycc+a01sURPmdE+plBS4UonGc0A7i6XeKAA)
+
+## Correctness
+We again want to show correctness for our `nbeT` algorithm, that is:
+
+`e ~ e' ↔ nbeT e = nbeT e'`
+
+While Soundness follows just like the Monoid-rewriting case (utilizing `convr_eval_eq`), Completeness (and more specifically `convr_nbe`)
+requires more to push-through.
+To show
+
+`e ~ nbeT e`
+
+we will utilize the method of Reducibility-candidates that we discussed earlier:
+```lean
+-- Tait-reducibility relation
+def R : (a : Ty) → (e : ExpT a) → Prop
+| Ty.Nat, e       => e ~ (nbeT Ty.Nat e)
+
+| Ty.arrow α β, e => e ~ (nbeT (α ⇒' β) e)  ∧  ∀ e', R α e' → R β (e ⬝ e')
+```
+Note that from this definition of Reducibility we get 3 trivial lemmas:
+```lean
+-- R a e  implies  e ~ nbeT a e
+theorem R_convr_nbe (h : R α e)  : e ~ (nbeT α e) :=
+  by
+  -- Hint: By cases on α
+  --  and def of R
+  sorry
+
+-- e ~ e' implies  R α e ↔ R α e'
+theorem convr_R_iff : ∀ e e' : ExpT α, e ~ e' → (R α e ↔ R α e') :=
+  by
+  -- Hint: Induction on α
+  --  and soundness
+  sorry
+
+theorem R_numeral : R Ty.Nat (numeral n) :=
+  by
+  -- Hint: Induction on n
+  sorry
+```
+[Try it!](https://live.lean-lang.org/#codez=LTAEDECcHsFsC5QAsAuKAOBneB6HBjTAOgEtp8iBTSnSgd00JwCYAGVgThwBMBPAIwBWlSDlgBDEgDsACuIA2sTJWCRKANxLLuRdNwBmAKBKx00SClABZcSiTyS/IgBVx+FCXyHjU7gFd3EnVKUGdeUEQw9EpDAB9QADlbCNDeONBxSBg6FLDQQCTCVILUw2hoqRLpfRIAD0gUgEZ2UAAiUEAlwgByVtAAXgA+DKzoOm9pf0Dg0ABRGvRc8MKomPiAaVAAb3FQfgWAX1BDw8QZudAACm2unY7u8QBKdIBlTe3d/H2jk9n588vbm7XfD3AH/a78EHXMHdYGPeIAQXQ8y2N0ivAOx0OPwuV26EOK2O2hWx/HSAC8RNAjtSaSlTvMkih0pgAh9abTvmdzoyAYy4aA1PgEq9Pl8sVzcRceddJQ9eckZY8ypQKj8fNUavJGs02oBcah6A1AiPQ3h8Ew8U3w0Ck6nqiEABcCbQCNwPsADQXbFOkGFc6e72gGQwE3xNT6LUbF1ovYbEKIT17QzslJWm31c6UEHp/mYXiwI4R/Yx0CUbpxs5OhNJxAp20XDN1zr+mtpkuZjPpFCQcRSTDOwshEvFzql+mgCuJ9nV621rMNpvTluNhtLwrNutt4f89bUguAJuBCzUUvHNuEy/Nd5XJ6A1+d1vrD/reJmavyXjuXfvAM3AUY2h7PF0/AF92uL0Dg2U9R3OQDrl3e4wLJI8zk/S8OWvBcLhee9QEfbDQDJZ9cIQ/VznCfV8P5cQkXzD9PhRXZ/3OYDulAzYPm4RDzxQmkp1THFM3xVd0POYELm4edeP+fURPOXZ9TE9JBQSAB9CkYD7KNNljUcK02fQOKlBVmIBUCJ1Qm9FNwkJ9T0sjKTbflFKUll8A+AsNI2Cp/0ZMCtOPDY9IY6UjJAuDTO4tCJIs/UrNAGyLmcj59Ske5MziipiKi4tcLSlL1VqbVWB6AA/A1BmbU1uEoPSwiU6QUBEBZimWdIwiIHlDUAVEJvHiTJsgyG5DWxaEdhBAB1i4arqhqiVSWqpHq+oIQqqqMiRZQ8zoz5zksNE5oWnEAQhDcFj26aQV2qbFoiXoLhQIhMF8IdHkMSq9KkPxYBEBQUh5Ykzlaxl0kKw1VOgdIpAAagaPpBgS3Dznez6uy1ZLvFegVKBIfRwn+NE2xOy6MnO0dtngXpDBwYAWt4NrbHdEIkyOQ1Ea+rUVlSIhepGfr+HdYT3X0EFDS8YAcEMfg0kOfBxGUXtxAnaXlESZJ2UNSgajcSwWeR4sFZlkIuZyN5DjVjX3GLIh9EwJk0ZWn5TrTUnUmJ9N9LlJZeAdjJ0gAAXWY3DVvV0wqTc5AG7gUB5kAMsILjvC41Cx8JtnQe5g8Zo5w9AABHUAY5TlL+R9l5jY+QOnjT9OM4jw8Y/OTD48x7GcS6fguhEl8K8ri4I/CWv6/OBOm8uFu25BF94cHnHxBbkEn07yvM4QmPKKwSg80uNa19AQ98JxTe83CciC9y+IfeNHnYqymHVtX9f7cJ4b8UFj05i97Z23iUH08DwrEA67NWTf0GOcBK88u5V1AJ5UAHVc6QKhiCQuFlti0kDopMB4Du6R1gQPSgQoJ6NyTpHVOIcMGZxzrXTKODE79RTvg6h3JbBdGnp0OUWdiEYJpJnKQhUY6MiIIKLBXCBSwJXutPet9s6QJBJAEE3Dj65Vtm9fgIRcbOzrG7F2hJzo3Unv1X0r9Cbv2eoYEAWUSqDlACYdADhKC9gANp2MoAAXScdsG6DiSwuPlvINeEgIq2iUhoBQgSc4oncgOEchIDiIBCOY7oPp9HoDfsWIWL8kmGKeto8WktLHzTUkgCc4wAgeGtMgCcCh5BKQAObQAUL2fAPjMj9QiaAcpUhPY1LqRkWxZQ9ZKxXmOUA+4S6gHYuIJSkAlLvAmUpMZ/BapIGvNwBZMMwp+CkPoaA8h2L33miIMKkAch2PEPMkgSB3T4GWWcpx3hTGxKHIcKxNjexSGUc0vokC3nv06IYHxsA/GYGgOs7gUhbG9jCakHyDz/ziGiWYh5hRXkGyyjdJFzTSzk0OBLCc6zNnbM+TER5eSqRIAaBOJA4gphIGYBxZJIQbq7P2t866/jJlBMqZQHOpKJyHNAHY6lNyTFgFcCQFAqhKATEcCQBwKBwhqHkLYMgUgXorQAEopFUWEf0rsYX+kDL0+IAM6ZXxpGrUAJUEZvKNZYds1NObDByB+em197mWpUS6GCIJ6ygEAOREhxAAAREOd06qXSDkKOq/crtoqNluWAdV79HmmGeYce5aL36GDsJQcwW9VVKWbEpNF5xFmIBDSkzErq0WhqyVinJpiAASdVEAACFwiK1saAUpToJymIyI9dG0A9KqonICrIaQhXwsHE8kg7bQClpCIAFMJZ2DJLBmpAWa1B5nzbmrGAVQCBoic6uJxRzhztAIuudS4yYTmxYcetjbQAAElfDFKVR2ioXbb1gF7exQFwLQWYEwIU59gRO0TgAO2gFxVs9iQ7qR1TUsbcZkzSTUhXvIcID79D6FIMSsKEH4NUiQwW5RJC73zUQAAVSVr+3w/7eylKIyhmkI7IA5M/aAJ4uZPqdk8NefWeHcmdipPMyZSKSEsbHYcCDagpDiE+rVQZ+4nQPrrUMlTYUCO9n0NDfQNLtMzN02FNDGGsM4aEwJgjs6lLaZIcZo0vgzMwBIRBsjKBEAkPY7FZgHnQCmKKj5ntNmkx+fThLKz2mcSPVzfmpFIIAtfrRUF9kpibqMzCzRkFYL4uHES95pMEnnOCbUoOVVK7gtgAbeR0AVGQi7hU6ATNFRc1JdpAV6kpjOP/MoDxj4baLPEvC3lmkdn4QOYI4VtrNIIMFdXeunNBaPqsxSOq61FxtbfWStda9taKv3qfeaV9pTlWHAk0AA)
+[Solution](https://live.lean-lang.org/#codez=LTAEDECcHsFsC5QAsAuKAOBneB6HBjTAOgEtp8iBTSnSgd00JwCYAGVgThwBMBPAIwBWlSDlgBDEgDsACuIA2sTJWCRKANxLLuRdNwBmAKBKx00SClABZcSiTyS/IgBVx+FCXyHjU7gFd3EnVKUGdeUEQw9EpDAB9QADlbCNDeONBxSBg6FLDQQCTCVILUw2hoqRLpfRIAD0gUgEZ2UAAiUEAlwgByVtAAXgA+DKzoOm9pf0Dg0ABRGvRc8MKomPiAaVAAb3FQfgWAX1BDw8QZudAACm2unY7u8QBKdIBlTe3d/H2jk9n588vbm7XfD3AH/a78EHXMHdYGPeIAQXQ8y2N0ivAOx0OPwuV26EOK2O2hWx/HSAC8RNAjtSaSlTvMkih0pgAh9abTvmdzoyAYy4aA1PgEq9Pl8sVzcRceddJQ9eckZY8ypQKj8fNUavJGs02oBcah6A1AiPQ3h8Ew8U3w0Ck6nqiEABcCbQCNwPsADQXbFOkGFc6e72gGQwE3xNT6LUbF1ovYbEKIT17QzslJWm31c6UEHp/mYXiwI4R/Yx0CUbpxs5OhNJxAp20XDN1zr+mtpkuZjPpFCQcRSTDOwshEvFzql+mgCuJ9nV621rMNpvTluNhtLwrNutt4f89bUguAJuBCzUUvHNuEy/Nd5XJ6A1+d1vrD/reJmavyXjuXfvAM3AUY2h7PF0/AF92uL0Dg2U9R3OQDrl3e4wLJI8zk/S8OWvBcLhee9QEfbDQDJZ9cIQ/VznCfV8P5cQkXzD9PhRXZ/3OYDulAzYPm4RDzxQmkp1THFM3xVd0POYELm4edeP+fURPOXZ9TE9JBQSAB9CkYD7KNNljUcK02fQOKlBVmIBUCJ1Qm9FNwkJ9T0sjKTbflFKUll8A+AsNI2Cp/0ZMCtOPDY9IY6UjJAuDTO4tCJIs/UrNAGyLmcj59Ske5MziipiKi4tcLSlL1VqbVWB6AA/A1BmbU1uEoPSwiU6QUBEBZimWdIwiIHlDUAVEJvHiTJsgyG5DWxaEdhBAB1i4arqhqiVSWqpHq+oIQqqqMiRZQ8zoz5zksNE5oWnEAQhDcFj26aQV2qbFoiXoLhQIhMF8IdHkMSq9KkPxYBEBQUh5Ykzlaxl0kKw1VOgdIpAAagaPpBgS3Dznez6uy1ZLvFegVKBIfRwn+NE2xOy6MnO0dtngXpDBwYAWt4NrbHdEIkyOQ1Ea+rUVlSIhepGfr+HdYT3X0EFDS8YAcEMfg0kOfBxGUXtxAnaXlESZJ2UNSgajcSwWeR4sFZlkIuZyN5DjVjX3GLIh9EwJk0ZWn5TrTUnUmJ9N9LlJZeAdjJ0gAAXWY3DVvV0wqTc5AG7gUB5kAMsILjvC41Cx8JtnQe5g8Zo5w9AABHUAY5TlL+R9l5jY+QOnjT9OM4jw8Y/OTD48x7GcS6fguhEl8K8ri4I/CWv6/OBOm8uFu25BF94cHnHxBbkEn07yvM4QmPKKwSg80uNa19AQ98JxTe83CciC9y+IfeNHnYqymHVtX9f7cJ4b8UFj05i97Z23iUH08DwrEA67NWTf0GOcBK88u5V1AJ5UAHVc6QKhiCQuFlti0kDopMB4Du6R1gQPSgQoJ6NyTpHVOIcMGZxzrXTKODE79RTvg6h3JbBdGnp0OUWdiEYJpJnKQhUY6MiIIKLBXCBSwJXutPet9s6QJBJAEE3Dj65Vtm9fgIRcbOzrG7F2hJzo3Unv1X0r9Cbv2eoYEAWUSqDlACYdADhKC9gANp2MoAAXScdsG6DiSwuPlvINeEgIq2iUhoBQgSc4oncgOEchIDiIBCOY7oPp9HoDfsWIWL8kmGKeto8WktLHzTUkgCc4wAgeGtMgCcCh5BKQAObQAUL2fAPjMj9QiaAcpUhPY1LqRkWxZQ9ZKxXmOUA+4S6gHYuIJSkAlLvAmUpMZ/BapIGvNwBZMMwp+CkPoaA8h2L33miIMKkAch2PEPMkgSB3T4GWWcpx3hTGxKHIcKxNjexSGUc0vokC3nv06IYHxsA/GYGgOs7gUhbG9jCakHyDz/ziGiWYh5hRXkGyyjdJFzTSzk0OBLCc6zNnbM+TER5eSqRIAaBOJA4gphIGYBxZJIQbq7P2t866/jJlBMqZQHOpKJyHNAHY6lNyTFgFcCQFAqhKATEcCQBwKBwhqHkLYMgUgXorQAEopFUWEf0rsYX+kDL0+IAM6ZXxpGrUAJUEZvKNZYds1NObDByB+em197mWpUS6GCIJ6ygEAOREhxAAAREOd06qXSDkKOq/crtoqNluWAdV79HmmGeYce5aL36GDsJQcwW9VVKWbEpNF5xFmIBDSkzErq0WhqyVinJitbFjnKfISpnT5C9nOLirZ7F42WCQPcAA3N0wFJohXwsHE8kg9bQClpCIAFMIp2DJLBmpAWa1B5nzbmrGAVQCBoic6uJxRzjTtAHO6dS4yYTmxUS80SqG2HAAO2gA7fi1VYU6pqWNuMyZpJqQr3kOEAAkvofQpBiVhQfW+qkn6C3KJIRSqYnKUhoutf1VFVqaY8nojdQFwLQWYDljM79nC1B0EgKKkIdjAAJhMWLOTj+3XkafUTlJDf3hGbEQTs3Y21QYhPdXMJD1aawyDMpFYVTFPFzJ9Tsnhrz6zA7kzsVJ5mTJE7SODA4c6ICQ+h5IbiCUcwwyy7DvhcP4a/SQnBJGyN8s5bRgdDTKBNKY7SAT5s2McZ7EJr9OxhMwYnA+tQUhxCfVqoM/cTp/0AAkhmRdfcS3s+hob6BpQlmZSWwosdAIB4DEG5MQanUpBLzGkR/qNL4EDCmSEPoy25rsHnzgpcmUl+4vHYAkMOGp6jiG3nnA9d0WCsVoaofdUBEESXDNAuM2CgbqXmBtYxpZ+qfKqM2bswx6jc2XOWFzfmtFubCu0nA8Sh5qrF1JkwNEfAJAFAkApNFqL9XobRtSjSp7FwGsFeYJzKibHQzyEeEmDLu5ItEFMHNyAdbex7ehnQUVizAAX5Epd0SBWCAEvyDbZse2FUHCdn51IxMScoFJj4dbctHb27N2kGX4RlZywdm+JWHszea+5zAc2OsIc0913rQzRuDb0z1kbsUaVk1AEZkFU33tpaTMR0ji3HE0dWw5xjWd0eCe2wuaDIRyeVfk2pbHp32TndwVdhwt2gf3YS5ZJc9WXtPTew0GbX35g/aqn9ubgPgemEgGDiH+Wxsw7sKABHSPUeq/Nsj47i6l0rpzQWj6rMUjquQwjePOtkrXQvTkp9XbCm+GKTe5VUt9Z4UpC6jHrL+Gu+8EXpWcMpDdEi6s6k2fIGp4UOl4rOMXdhmayvMKm3MsRaAA)
+
+With these results in place, we are now ready to prove our main lemma, that all Godel-T terms are reducible:
+
+`∀ e : ExpT α, R α e`
+
+Since this is such an intergral lemma to our correctness proof, we will walk through this proof for the case where `e = recN`
+(since all other cases are similar to this one).
+
+```lean
+example (α : Ty) :  R (α ⇒' (Ty.Nat ⇒' α ⇒' α) ⇒' Ty.Nat ⇒' α) .recN :=
+by
+-- By def of `R` we must prove two things:
+apply And.intro
+
+-- `recN ~ (nbeT (α ⇒' (Ty.Nat ⇒' α ⇒' α) ⇒' Ty.Nat ⇒' α) recN):`
+-- Since `nbeT recN = recN`, this follows by `convrT.refl`.
+· exact convrT.refl
+
+-- `∀ e', R α e' → R ((Ty.Nat ⇒' α ⇒' α) ⇒' Ty.Nat ⇒' α) (recN ⬝ e'):`
+-- Suppose we have `R α e'`, by def of `R` we must prove two things:
+· intro e' Re'
+  apply And.intro
+
+  -- `recN ⬝ e' ~ nbeT ((Ty.Nat ⇒' α ⇒' α) ⇒' Ty.Nat ⇒' α) (recN ⬝ e'):`
+  -- Since `nbeT (recN ⬝ e') = recN ⬝ (nbeT e')`, this follows by `R α e'`.
+  · have eq : nbeT ((Ty.Nat ⇒' α ⇒' α) ⇒' Ty.Nat ⇒' α) (.recN ⬝ e') = .recN ⬝ nbeT α e' := rfl; rewrite [eq]; clear eq
+    apply convrT.app convrT.refl
+    exact R_convr_nbe Re'
+
+  -- `∀ e'', R (Ty.Nat ⇒' α ⇒' α) e'' → R (Ty.Nat ⇒' α) (recN ⬝ e' ⬝ e''):`
+  -- Suppose we have `R (Ty.Nat ⇒' α ⇒' α) e''`, by def of `R` we must prove two things:
+  · intro e'' Re''
+    apply And.intro
+
+    --`(recN ⬝ e' ⬝ e'') ~ nbeT (Ty.Nat ⇒' α) (recN ⬝ e' ⬝ e''):`
+    -- Since `nbeT (recN ⬝ e' ⬝ e'') = recN ⬝ (nbeT e') ⬝ (nbeT e'')`, this follows by `R α e'` and `R (Ty.Nat ⇒' α ⇒' α) e''`.
+    · have eq : nbeT (Ty.Nat ⇒' α) (.recN ⬝ e' ⬝ e'') = .recN ⬝ nbeT α e' ⬝ nbeT (Ty.Nat ⇒' α ⇒' α) e'' := rfl; rewrite [eq]; clear eq
+      replace Re' := R_convr_nbe Re'; replace Re'' := R_convr_nbe Re''
+      have h0 : convrT (.recN ⬝ e') (.recN ⬝ nbeT α e') := (convrT.refl).app Re'
+      exact h0.app Re''
+
+    -- `∀ n, R (Ty.Nat) n → R α (recN ⬝ e' ⬝ e'' ⬝ n):`
+    -- Suppose we have `R (Ty.Nat) n`, by def of `R` we have `n ~ nbeT n` so by `convr_R_iff` suffices to show:
+    --      `R α (recN ⬝ e' ⬝ e'' ⬝ (nbeT n)):`
+    -- Since `nbeT n = numeral [[n]]`, we may perform induction on `[[n]] : ℕ`:
+    · intro n Rn
+      have convr_n := Rn
+      unfold R at convr_n
+      apply (convr_R_iff (.recN ⬝ e' ⬝ e'' ⬝ n) (.recN ⬝ e' ⬝ e'' ⬝ (nbeT Ty.Nat n)) (convrT.refl.app Rn)).mpr
+      unfold nbeT; simp [reifyT]
+      induction ((ExpT_inter Ty.Nat n))
+
+      -- `R α (recN ⬝ e' ⬝ e'' ⬝ (numeral 0)):`
+      -- By `convr_R_iff` and `R α e'` we are done.
+      · unfold numeral
+        exact (convr_R_iff (.recN ⬝ e' ⬝ e'' ⬝ .zero) e' convrT.recN_zero).mpr Re'
+
+      -- `R α (recN ⬝ e' ⬝ e'' ⬝ (numeral (n'+1))):` By def of `numeral` and `convr_R_iff`, suffices to show:
+      --     ` R α (e'' ⬝ numeral n' ⬝ (recN ⬝ e' ⬝ e'' ⬝ numeral n')):`
+      -- By `R (Ty.Nat ⇒' α ⇒' α) e''`, `R_numeral`, and `IH` we are done.
+      · rename_i n' IH
+        apply (convr_R_iff (.recN ⬝ e' ⬝ e'' ⬝ (.succ ⬝ numeral n')) (e'' ⬝ (numeral n') ⬝ (.recN ⬝ e' ⬝ e'' ⬝ (numeral n'))) convrT.recN_succ).mpr
+        have R_numeral_n' : R Ty.Nat (numeral n') := by exact R_numeral
+        rcases Re'' with ⟨_, h0⟩
+        specialize h0 (numeral n') R_numeral_n'
+        rcases h0 with ⟨_, h0⟩
+        exact h0 (.recN ⬝ e' ⬝ e'' ⬝ numeral n') IH
+```
+[Example on Lean4 web server](https://live.lean-lang.org/#codez=LTAEDECcHsFsC5QAsAuKAOBneB6HBjTAOgEtp8iBTSnSgd00JwCYAGVgThwBMBPAIwBWlSDlgBDEgDsACuIA2sTJWCRKANxLLuRdNwBmAKBKx00SClABZcSiTyS/IgBVx+FCXyHjU7gFd3EnVKUGdeUEQw9EpDAB9QADlbCNDeONBxSBg6FLDQQCTCVILUw2hoqRLpfRIAD0gUgEZ2UAAiUEAlwgByVtAAXgA+DKzoOm9pf0Dg0ABRGvRc8MKomPiAaVAAb3FQfgWAX1BDw8QZudAACm2unY7u8QBKdIBlTe3d/H2jk9n588vbm7XfD3AH/a78EHXMHdYGPeIAQXQ8y2N0ivAOx0OPwuV26EOK2O2hWx/HSAC8RNAjtSaSlTvMkih0pgAh9abTvmdzoyAYy4aA1PgEq9Pl8sVzcRceddJQ9eckZY8ypQKj8fNUavJGs02oBcah6A1AiPQ3h8Ew8U3w0Ck6nqiEABcCbQCNwPsADQXbFOkGFc6e72gGQwE3xNT6LUbF1ovYbEKIT17QzslJWm31c6UEHp/mYXiwI4R/Yx0CUbpxs5OhNJxAp20XDN1zr+mtpkuZjPpFCQcRSTDOwshEvFzql+mgCuJ9nV621rMNpvTluNhtLwrNutt4f89bUguAJuBCzUUvHNuEy/Nd5XJ6A1+d1vrD/reJmavyXjuXfvAM3AUY2h7PF0/AF92uL0Dg2U9R3OQDrl3e4wLJI8zk/S8OWvBcLhee9QEfbDQDJZ9cIQ/VznCfV8P5cQkXzD9PhRXZ/3OYDulAzYPm4RDzxQmkp1THFM3xVd0POYELm4edeP+fURPOXZ9TE9JBQSAB9CkYD7KNNljUcK02fQOKlBVmIBUCJ1Qm9FNwkJ9T0sjKTbflFKUll8A+AsNI2Cp/0ZMCtOPDY9IY6UjJAuDTO4tCJIs/UrNAGyLmcj59Ske5MziipiKi4tcLSlL1VqbVWB6AA/A1BmbU1uEoPSwiU6QUBEBZimWdIwiIHlDUAVEJvHiTJsgyG5DWxaEdhBAB1i4arqhqiVSWqpHq+oIQqqqMiRZQ8zoz5zksNE5oWnEAQhDcFj26aQV2qbFoiXoLhQIhMF8IdHkMSq9KkPxYBEBQUh5Ykzlaxl0kKw1VOgdIpAAagaPpBgS3Dznez6uy1ZLvFegVKBIfRwn+NE2xOy6MnO0dtngXpDBwYAWt4NrbHdEIkyOQ1Ea+rUVlSIhepGfr+HdYT3X0EFDS8YAcEMfg0kOfBxGUXtxAnaXlESZJ2UNSgajcSwWeR4sFZlkIuZyN5DjVjX3GLIh9EwJk0ZWn5TrTUnUmJ9N9LlJZeAdjJ0gAAXWY3DVvV0wqTc5AG7gUB5kAMsILjvC41Cx8JtnQe5g8Zo5w9AABHUAY5TlL+R9l5jY+QOnjT9OM4jw8Y/OTD48x7GcS6fguhEl8K8ri4I/CWv6/OBOm8uFu25BF94cHnHxBbkEn07yvM4QmPKKwSg80uNa19AQ98JxTe83CciC9y+IfeNHnYqymHVtX9f7cJ4b8UFj05i97Z23iUH08DwrEA67NWTf0GOcBK88u5V1AJ5UAHVc6QKhiCQuFlti0kDopMB4Du6R1gQPSgQoJ6NyTpHVOIcMGZxzrXTKODE79RTvg6h3JbBdGnp0OUWdiEYJpJnKQhUY6MiIIKLBXCBSwJXutPet9s6QJBJAEE3Dj65Vtm9fgIRcbOzrG7F2hJzo3Unv1X0r9Cbv2eoYEAWUSqDlACYdADhKC9gANp2MoAAXScdsG6DiSwuPlvINeEgIq2iUhoBQgSc4oncgOEchIDiIBCOY7oPp9HoDfsWIWL8kmGKeto8WktLHzTUkgCc4wAgeGtMgCcCh5BKQAObQAUL2fAPjMj9QiaAcpUhPY1LqRkWxZQ9ZKxXmOUA+4S6gHYuIJSkAlLvAmUpMZ/BapIGvNwBZMMwp+CkPoaA8h2L33miIMKkAch2PEPMkgSB3T4GWWcpx3hTGxKHIcKxNjexSGUc0vokC3nv06IYHxsA/GYGgOs7gUhbG9jCakHyDz/ziGiWYh5hRXkGyyjdJFzTSzk0OBLCc6zNnbM+TER5eSqRIAaBOJA4gphIGYBxZJIQbq7P2t866/jJlBMqZQHOpKJyHNAHY6lNyTFgFcCQFAqhKATEcCQBwKBwhqHkLYMgUgXorQAEopFUWEf0rsYX+kDL0+IAM6ZXxpGrUAJUEZvKNZYds1NObDByB+em197mWpUS6GCIJ6ygEAOREhxAAAREOd06qXSDkKOq/crtoqNluWAdV79HmmGeYce5aL36GDsJQcwW9VVKWbEpNF5xFmIBDSkzErq0WhqyVinJitbFjnKfISpnT5C9nOLirZ7F42WCQPcAA3N0wFJohXwsHE8kg9bQClpCIAFMIp2DJLBmpAWa1B5nzbmrGAVQCBoic6uJxRzjTtAHO6dS4yYTmxUS80SqG2HAAO2gA7fi1VYU6pqWNuMyZpJqQr3kOEAAkvofQpBiVhQfW+qkn6C3KJIRSqYnKUhoutf1VFVqaY8nojdQFwLQWYDljM79nC1B0EgKKkIdjAAJhMWLOTj+3XkafUTlJDf3hGbEQTs3Y21QYhPdXMJD1aawyDMpFYVTFPFzJ9Tsnhrz6zA7kzsVJ5mTJE7SODA4c6ICQ+h5IbiCUcwwyy7DvhcP4a/SQnBJGyN8s5bRgdDTKBNKY7SAT5s2McZ7EJr9OxhMwYnA+tQUhxCfVqoM/cTp/0AAkhmRdfcS3s+hob6BpQlmZSWwosdAIB4DEG5MQanUpBLzGkR/qNL4EDCmSEPoy25rsHnzgpcmUl+4vHYAkMOGp6jiG3nnA9d0WCsVoaofdUBEESXDNAuM2CgbqXmBtYxpZ+qfKqM2bswx6jc2XOWFzfmtFubCu0nA8Sh5qrF1JkwNEfAJAFAkApNFqL9XobRtSjSp7FwGsFeYJzKibHQzyEeEmDLu5ItEFMHNyAdbex7ehnQUVizAAX5Epd0SBWCAEvyDbZse2FUHCdn51IxMScoFJj4dbctHb27N2kGX4RlZywdm+JWHszea+5zAc2OsIc0913rQzRuDb0z1kbsUaVk1AEZkFU33tpaTMR0ji3HE0dWw5xjWd0eCe2wuaDIRyeVfk2pbHp32TndwVdhwt2gf3YS5ZJc9WXtPTew0GbX35g/aqn9ubgPgemEgGDiH+Wxsw7sKABHSPUeq/Nsj47i6l0rpzQWj6rMUjquQwjePOtkrXQvTkp9XbCm+GKTe5VUt9Z4UpC6jHrL+Gu+8EXpWcMpDdEi6s6k2fIGp4UOl4rOMXdhmayvMKm3MsRdjRjPBWgMaSv4D4wwAmk3DbxnSdVAuoTIZAsZSE3QV/MWkbg4U57sWmIAELhHRtAPSAADVVZ/QB0BCLAPw1tI4wCmCgOgVI7DSCqdgQwVOaegZHWfiyC1Qtbnc4TfQZEKAEMAr0EfBIe4eAM/EdJ4aQfAEIM/NFCyHRHfM/d0d/eLLZeQEYXsCWUAM/bveQM/IgQwB9AfMg4fM/HdToYNBdeJedP4KAtfSA7TSwCAnBPBJ7eAxAvwJEaAJWG/ZASlVA09bAnYY/FaU/Egy/a/W/e/SwdAJ/EIF/N/JAD/L/Q7BTSPXHencIanHQHLCcUxAAnfK3c1fnUArg4yDg64KAzMTKVsAQw4MTZA1AwtVwpcTAvgi4NFVsaQ3A2KfAwgmQhQ5gigvzcQ+DDTWw9giApw+wng3w1JTKStaFHRMMAdGXKzeXJxRXRzFXH9TvCvAZWg6kAfdXVMTXKdKPDwsAegocRg1gpIrfVo4oRfZwhuAIwcaNRsdw0AMTIQswUQkIDrC/CaVI4KToksToaQ4gk/c/RQsQu/B/NQ6AZ/V/UAd/KQT/eAWIvLBYho4cDvaxYw3/CrUTYAM/Xg4UaNK3JcEqQtXoh46wwYuAhAvHMAJAqQFAkgnwqwp4r4j5ShIIpcYiSExsEI7QvAptCI4g6Y0NRYjIR6aYuw2mbguYscL1YcGI6kB9dnBIt42YvEvox4h5ME/wqkrIgY/nDoik04kXSAXI+bWXcjFbejJXdbWkNQaxNwLXQcEXWogJXbEsPIygQUwEnHDFfLHbN5OU2DCQ5AX+VlSkq3FwkEvTVE7RC4Mg3vKiHHfjcvZHJ3M4n5W4kgwNKQJgrEvkSBbowZD40EropKb460p4MYkQkIMQqYnorg2RJY2QvSeQi/K/f01UtAmwtFKQK/QFSI0gjXDdIDBMvwIDTwetFAKkTAJAEYI4342kFEzUt0046Et5ZKT0os/4wEtAysj5bWb6BxKQFxaQ9Y8QcIaINk8wPMIpQIUpUpM/FslxFIDqM/Qso4PQtSCoVVQvGkDrHbFlOckhFvbtVlAtIrS4g0lM2qIDUs6k90qRA8hk8swItDbEqRTMMgi0uclKEHNQ1cjZTtAlAdTAKxPlSeG5WkfskpCoP4RlBqZDKs6vGkCw0tV0w8s8lPJGb6VgFKYYoso/Eg9dPc/QK/bsdiEsksSMg2NQUZa0SgSgunFvJs+QMPSwYSXczdE87oQYwiOyB5F3IUFSOyB8+oE0khcCl03w54+GMiwIzoeBBCq/ZClYoEtvcg9ErC1CzdaQlkTMlA3sHM0XfMugScos6kK/CCs8gS+vfBfouio8vSxsassCsAZCzEpk6AhY6Qi/OPWC8g90TCkgyLXCoYEIbgQi4imkfzFUILSgELfSmLAHcoqiuo1MvSSC084ceGOGJKSSyBUy5cfixK+vEEDKHUmKoymChPdKlKCvRyBKZrL3NnVU3NMigtEcJPew3KtPM9G6Ygmohy1mH3fWSHU4gPeHRHNUtHM7C7E3G7SYwqOq76dK/LSq+vNq2WNU6/WHIPHq5HPq9kAfCPaKoy3StKpcSLIAA)
+
+With similar reasoning for the other cases, we get our Reducibility proof:
+
+```lean
+-- for all e, R a e
+theorem all_R {e : ExpT α} : R α e :=
+  by
+  sorry
+```
+[Try it!](https://live.lean-lang.org/#codez=LTAEDECcHsFsC5QAsAuKAOBneB6HBjTAOgEtp8iBTSnSgd00JwCYAGVgThwBMBPAIwBWlSDlgBDEgDsACuIA2sTJWCRKANxLLuRdNwBmAKBKx00SClABZcSiTyS/IgBVx+FCXyHjU7gFd3EnVKUGdeUEQw9EpDAB9QADlbCNDeONBxSBg6FLDQQCTCVILUw2hoqRLpfRIAD0gUgEZ2UAAiUEAlwgByVtAAXgA+DKzoOm9pf0Dg0ABRGvRc8MKomPiAaVAAb3FQfgWAX1BDw8QZudAACm2unY7u8QBKdIBlTe3d/H2jk9n588vbm7XfD3AH/a78EHXMHdYGPeIAQXQ8y2N0ivAOx0OPwuV26EOK2O2hWx/HSAC8RNAjtSaSlTvMkih0pgAh9abTvmdzoyAYy4aA1PgEq9Pl8sVzcRceddJQ9eckZY8ypQKj8fNUavJGs02oBcah6A1AiPQ3h8Ew8U3w0Ck6nqiEABcCbQCNwPsADQXbFOkGFc6e72gGQwE3xNT6LUbF1ovYbEKIT17QzslJWm31c6UEHp/mYXiwI4R/Yx0CUbpxs5OhNJxAp20XDN1zr+mtpkuZjPpFCQcRSTDOwshEvFzql+mgCuJ9nV621rMNpvTluNhtLwrNutt4f89bUguAJuBCzUUvHNuEy/Nd5XJ6A1+d1vrD/reJmavyXjuXfvAM3AUY2h7PF0/AF92uL0Dg2U9R3OQDrl3e4wLJI8zk/S8OWvBcLhee9QEfbDQDJZ9cIQ/VznCfV8P5cQkXzD9PhRXZ/3OYDulAzYPm4RDzxQmkp1THFM3xVd0POYELm4edeP+fURPOXZ9TE9JBQSAB9CkYD7KNNljUcK02fQOKlBVmIBUCJ1Qm9FNwkJ9T0sjKTbflFKUll8A+AsNI2Cp/0ZMCtOPDY9IY6UjJAuDTO4tCJIs/UrNAGyLmcj59Ske5MziipiKi4tcLSlL1VqbVWB6AA/A1BmbU1uEoPSwiU6QUBEBZimWdIwiIHlDUAVEJvHiTJsgyG5DWxaEdhBAB1i4arqhqiVSWqpHq+oIQqqqMiRZQ8zoz5zksNE5oWnEAQhDcFj26aQV2qbFoiXoLhQIhMF8IdHkMSq9KkPxYBEBQUh5Ykzlaxl0kKw1VOgdIpAAagaPpBgS3Dznez6uy1ZLvFegVKBIfRwn+NE2xOy6MnO0dtngXpDBwYAWt4NrbHdEIkyOQ1Ea+rUVlSIhepGfr+HdYT3X0EFDS8YAcEMfg0kOfBxGUXtxAnaXlESZJ2UNSgajcSwWeR4sFZlkIuZyN5DjVjX3GLIh9EwJk0ZWn5TrTUnUmJ9N9LlJZeAdjJ0gAAXWY3DVvV0wqTc5AG7gUB5kAMsILjvC41Cx8JtnQe5g8Zo5w9AABHUAY5TlL+R9l5jY+QOnjT9OM4jw8Y/OTD48x7GcS6fguhEl8K8ri4I/CWv6/OBOm8uFu25BF94cHnHxBbkEn07yvM4QmPKKwSg80uNa19AQ98JxTe83CciC9y+IfeNHnYqymHVtX9f7cJ4b8UFj05i97Z23iUH08DwrEA67NWTf0GOcBK88u5V1AJ5UAHVc6QKhiCQuFlti0kDopMB4Du6R1gQPSgQoJ6NyTpHVOIcMGZxzrXTKODE79RTvg6h3JbBdGnp0OUWdiEYJpJnKQhUY6MiIIKLBXCBSwJXutPet9s6QJBJAEE3Dj65Vtm9fgIRcbOzrG7F2hJzo3Unv1X0r9Cbv2eoYEAWUSqDlACYdADhKC9gANp2MoAAXScdsG6DiSwuPlvINeEgIq2iUhoBQgSc4oncgOEchIDiIBCOY7oPp9HoDfsWIWL8kmGKeto8WktLHzTUkgCc4wAgeGtMgCcCh5BKQAObQAUL2fAPjMj9QiaAcpUhPY1LqRkWxZQ9ZKxXmOUA+4S6gHYuIJSkAlLvAmUpMZ/BapIGvNwBZMMwp+CkPoaA8h2L33miIMKkAch2PEPMkgSB3T4GWWcpx3hTGxKHIcKxNjexSGUc0vokC3nv06IYHxsA/GYGgOs7gUhbG9jCakHyDz/ziGiWYh5hRXkGyyjdJFzTSzk0OBLCc6zNnbM+TER5eSqRIAaBOJA4gphIGYBxZJIQbq7P2t866/jJlBMqZQHOpKJyHNAHY6lNyTFgFcCQFAqhKATEcCQBwKBwhqHkLYMgUgXorQAEopFUWEf0rsYX+kDL0+IAM6ZXxpGrUAJUEZvKNZYds1NObDByB+em197mWpUS6GCIJ6ygEAOREhxAAAREOd06qXSDkKOq/crtoqNluWAdV79HmmGeYce5aL36GDsJQcwW9VVKWbEpNF5xFmIBDSkzErq0WhqyVinJitbFjnKfISpnT5C9nOLirZ7F42WCQPcAA3N0wFJohXwsHE8kg9bQClpCIAFMIp2DJLBmpAWa1B5nzbmrGAVQCBoic6uJxRzjTtAHO6dS4yYTmxUS80SqG2HAAO2gA7fi1VYU6pqWNuMyZpJqQr3kOEAAkvofQpBiVhQfW+qkn6C3KJIRSqYnKUhoutf1VFVqaY8nojdQFwLQWYDljM79nC1B0EgKKkIdjAAJhMWLOTj+3XkafUTlJDf3hGbEQTs3Y21QYhPdXMJD1aawyDMpFYVTFPFzJ9Tsnhrz6zA7kzsVJ5mTJE7SODA4c6ICQ+h5IbiCUcwwyy7DvhcP4a/SQnBJGyN8s5bRgdDTKBNKY7SAT5s2McZ7EJr9OxhMwYnA+tQUhxCfVqoM/cTp/0AAkhmRdfcS3s+hob6BpQlmZSWwosdAIB4DEG5MQanUpBLzGkR/qNL4EDCmSEPoy25rsHnzgpcmUl+4vHYAkMOGp6jiG3nnA9d0WCsVoaofdUBEESXDNAuM2CgbqXmBtYxpZ+qfKqM2bswx6jc2XOWFzfmtFubCu0nA8Sh5qrF1JkwNEfAJAFAkApNFqL9XobRtSjSp7FwGsFeYJzKibHQzyEeEmDLu5ItEFMHNyAdbex7ehnQUVizAAX5Epd0SBWCAEvyDbZse2FUHCdn51IxMScoFJj4dbctHb27N2kGX4RlZywdm+JWHszea+5zAc2OsIc0913rQzRuDb0z1kbsUaVk1AEZkFU33tpaTMR0ji3HE0dWw5xjWd0eCe2wuaDIRyeVfk2pbHp32TndwVdhwt2gf3YS5ZJc9WXtPTew0GbX35g/aqn9ubgPgemEgGDiH+Wxsw7sKABHSPUeq/Nsj47i6l0rpzQWj6rMUjquQwjePOtkrXQvTkp9XbCm+GKTe5VUt9Z4UpC6jHrL+Gu+8EXpWcMpDdEi6s6k2fIGp4UOl4rOMXdhmayvMKm3MsRdjbFcwGQm3FmDc035vjtgVKUuqosMK4Xxqyuemtufr2lMJWP5ttTW30aV97GvIR/YDX6KJsAAAhcI6NoB6QAAaqvv6AOgIRYB+GtpHGAUwUB0CpHYaQKpbADvaxcIanHQWnI4UxCLOqRAAAdRCA63vzRXWBulWHvzk0BSyByUOFJwU0j1xxpDEz8CRGgCVlf2QEpRCEfwXU6Hv3dAllGRWjv1AEf2fwoPf0/3QG/xCF/3/yQEAOAMp071KwgNAzp2gNgNAAiyoNADsGSGQO6zjlbA+TjjRRLAwKTFMWv1YNPXYINjUFGWtEoCIDmywMgBwKOAfUkPmngIMJCG4GMJ2HCHv3XVqiA3oNYLY3QPdG7HYkfw0LmzyxLG6CUjMPMAsOrxkyVmLhuFLnPzxyvxv2YIfyfxfzfw/0sG4OgB/z/zkIEKkCAPgBAJK3APKxgAv2kKkIQMoKmEUJCBeBuieE0KsNFwiMsLwLUkPFVRqBIWINIPIMQNkJoMfgBBEm3k8MYNv1SP0NAE4KyJ4LkLyIAMKKEJpCpxp3EJpGsLABgNsOkNkPkMsHqIwlwnHiaPhjRRfBaNpFMWcGXQqAoMyAcKcMYMfxqHv1MLO3aJ1zy3CFVUsMSKeBILMEGNqOoPVUflnkmOSL0hYLYPSLmMyK/xyN4OWIKKKPdxELKMgIkN2KkJkLqMLXrgfFACfA+XriuNwjRV4BuPZDuIeMROeKMNBWcN0I+IyEekf1pKIFaXTnMMBNaJsJQEQAAFUlZXCNcN0PDOT/C2Nmi5CqQ1AJheDl1QAW1FTij05TEaQaCPhzhSSiILhSI8IUo6TbjhVGSP8ISPj3RuTPC/DdCyRn8UAqRqgpAtBFlM0US79eS5siV8CEJVUyR/S2jsCoi60jQqIaI9Jui9Ieim8oD8T9jxSIT9B2DYd2S6SBSIzi8v4BhKi9iRTQAdDpjdDsyfi+kQg4YCzEiSzYTQB4S0iODkTsjcj+DBCtSjgNixCKs6yizEBCTqC0UazRdWQ6SH0czqQ5NhTBzhjC04Z7xUlFyLgriQRzTQAGSVRH0JSeiNy8tujejaQcyqyMY8EXRaykz6ymC4SZjET5iUT2z8jOySiwDNiKtKj78LILVC1udzhkMQJjJIRugALmJpFcEEh7h4A6SxNpB8Bhy3kLIdEILPCAD4stl5ARhew3ju95BPi5MB9cKojDhTF78d1OhJ9Q14l50/hQLBkQoAQ6KvQG48EntoLKjgSBiQgKCkC9CGCGymzZiHy2y0SOzViuz71dcqR9dCCf1sT3yKi+iwAvyIKrdzV+d/ztNLBAKGLrgmLMxMpWx2KLTQAng4KEKVFDKlxkLWLVy3lWxUKBD0Km0sK2SaCqL8K6d2cNMNKmKgLGKtL/KcFbKVCbLhQko3kqKWVIAwwB0ZcrN5cnFFdHMVcAcRC2MBkiKkwB91dUxNcp0o8TKyKhwKKaK/KGKQjihIT9KWLwqHlo1GxjKiCwBOLQTuKhi6jqrAqdKwKSqYSbzGy7yWyuDFi+DnzxLfijtKqcdZL1j5LezFKtDgB79gq6rBwGqQQSpC0arVq1KNqmqTKzKpB4LWDC0rKrdrKzy6q3U7diJ1DNxHKtAR8XKGA3K9DZTdCJpurgpeqQjPL2QH1vKusVEdrzqNqPlMpK16r+dyrfrhxorYr5tZdyMVsD8UrQy1BrE3AtdBwRdcqAldsSw4rKAsaTqZqWV8blM3kZrQyOsI8eIZwrKDLVKIqQgqLtELhcLe8qIcdQyB9kcncCrhxiLmrWDA0pBJ9NLaYUBZEqrBldro0LrqSoKNySKWqQSyD2rwTPqpa+RIF+qyyESeL5z1K0UpBn9AU3K3DN0La/AgNPB61XTRckARgJLRbdTS0FbobKq7q3lkoVa5tYLjqLLIEPltZvoHEpAXFPCODxBwhogYrzA8wilAhSlSl79I6XEUgOp783bqRDt8CKhVVC9GYOsdsKaS6kwW9u1WUC1QyMthIpT3C9Ivb1qSrlbaq9r27faQhkN/bOaFxK8wxBbi6UoQduDQyW8kUB1MArE+VJ4bl04U6SkKg/hGUGo+6FFtTlLPawbu7Vy28tRWAUoDr6SkivCm6baPr3KhxZjmTHDQUvjGYH0p7D7QyU1y9G68rpSW696faS8YAvUYRB7HJQZmsvchaRaird6Wbvb4a7rD7VzOh4ET7n9SyUjTrD7n9HTJTv7m7PCWR7b4LewnbMAXa6A873ajhn9Pb/7w6UZugMpYG266HEH69UHQztCXCurpbjJ/K/q7Tc16GHSuTIs77DCH6TDQz/MVQgtKAQt69B9376cu9L6gNO7FaGr4YVz6HIFGwNxGGD6kZvp2H8EQrDH/6U9jGGGC4K9HIEpwGJ6u4OshHD6C0Rwk9AqrGE9TGRdGCcq49rHlHwd9ZIdKqA94dEdkBQ8u4jdLtrtbsI9vG08lxXHrH3HgnfcI8Img8onkc0cu5+bCpW6LH4HW9rG9GQRIsgA)
+[Solution](https://live.lean-lang.org/#codez=LTAEDECcHsFsC5QAsAuKAOBneB6HBjTAOgEtp8iBTSnSgd00JwCYAGVgThwBMBPAIwBWlSDlgBDEgDsACuIA2sTJWCRKANxLLuRdNwBmAKBKx00SClABZcSiTyS/IgBVx+FCXyHjU7gFd3EnVKUGdeUEQw9EpDAB9QADlbCNDeONBxSBg6FLDQQCTCVILUw2hoqRLpfRIAD0gUgEZ2UAAiUEAlwgByVtAAXgA+DKzoOm9pf0Dg0ABRGvRc8MKomPiAaVAAb3FQfgWAX1BDw8QZudAACm2unY7u8QBKdIBlTe3d/H2jk9n588vbm7XfD3AH/a78EHXMHdYGPeIAQXQ8y2N0ivAOx0OPwuV26EOK2O2hWx/HSAC8RNAjtSaSlTvMkih0pgAh9abTvmdzoyAYy4aA1PgEq9Pl8sVzcRceddJQ9eckZY8ypQKj8fNUavJGs02oBcah6A1AiPQ3h8Ew8U3w0Ck6nqiEABcCbQCNwPsADQXbFOkGFc6e72gGQwE3xNT6LUbF1ovYbEKIT17QzslJWm31c6UEHp/mYXiwI4R/Yx0CUbpxs5OhNJxAp20XDN1zr+mtpkuZjPpFCQcRSTDOwshEvFzql+mgCuJ9nV621rMNpvTluNhtLwrNutt4f89bUguAJuBCzUUvHNuEy/Nd5XJ6A1+d1vrD/reJmavyXjuXfvAM3AUY2h7PF0/AF92uL0Dg2U9R3OQDrl3e4wLJI8zk/S8OWvBcLhee9QEfbDQDJZ9cIQ/VznCfV8P5cQkXzD9PhRXZ/3OYDulAzYPm4RDzxQmkp1THFM3xVd0POYELm4edeP+fURPOXZ9TE9JBQSAB9CkYD7KNNljUcK02fQOKlBVmIBUCJ1Qm9FNwkJ9T0sjKTbflFKUll8A+AsNI2Cp/0ZMCtOPDY9IY6UjJAuDTO4tCJIs/UrNAGyLmcj59Ske5MziipiKi4tcLSlL1VqbVWB6AA/A1BmbU1uEoPSwiU6QUBEBZimWdIwiIHlDUAVEJvHiTJsgyG5DWxaEdhBAB1i4arqhqiVSWqpHq+oIQqqqMiRZQ8zoz5zksNE5oWnEAQhDcFj26aQV2qbFoiXoLhQIhMF8IdHkMSq9KkPxYBEBQUh5Ykzlaxl0kKw1VOgdIpAAagaPpBgS3Dznez6uy1ZLvFegVKBIfRwn+NE2xOy6MnO0dtngXpDBwYAWt4NrbHdEIkyOQ1Ea+rUVlSIhepGfr+HdYT3X0EFDS8YAcEMfg0kOfBxGUXtxAnaXlESZJ2UNSgajcSwWeR4sFZlkIuZyN5DjVjX3GLIh9EwJk0ZWn5TrTUnUmJ9N9LlJZeAdjJ0gAAXWY3DVvV0wqTc5AG7gUB5kAMsILjvC41Cx8JtnQe5g8Zo5w9AABHUAY5TlL+R9l5jY+QOnjT9OM4jw8Y/OTD48x7GcS6fguhEl8K8ri4I/CWv6/OBOm8uFu25BF94cHnHxBbkEn07yvM4QmPKKwSg80uNa19AQ98JxTe83CciC9y+IfeNHnYqymHVtX9f7cJ4b8UFj05i97Z23iUH08DwrEA67NWTf0GOcBK88u5V1AJ5UAHVc6QKhiCQuFlti0kDopMB4Du6R1gQPSgQoJ6NyTpHVOIcMGZxzrXTKODE79RTvg6h3JbBdGnp0OUWdiEYJpJnKQhUY6MiIIKLBXCBSwJXutPet9s6QJBJAEE3Dj65Vtm9fgIRcbOzrG7F2hJzo3Unv1X0r9Cbv2eoYEAWUSqDlACYdADhKC9gANp2MoAAXScdsG6DiSwuPlvINeEgIq2iUhoBQgSc4oncgOEchIDiIBCOY7oPp9HoDfsWIWL8kmGKeto8WktLHzTUkgCc4wAgeGtMgCcCh5BKQAObQAUL2fAPjMj9QiaAcpUhPY1LqRkWxZQ9ZKxXmOUA+4S6gHYuIJSkAlLvAmUpMZ/BapIGvNwBZMMwp+CkPoaA8h2L33miIMKkAch2PEPMkgSB3T4GWWcpx3hTGxKHIcKxNjexSGUc0vokC3nv06IYHxsA/GYGgOs7gUhbG9jCakHyDz/ziGiWYh5hRXkGyyjdJFzTSzk0OBLCc6zNnbM+TER5eSqRIAaBOJA4gphIGYBxZJIQbq7P2t866/jJlBMqZQHOpKJyHNAHY6lNyTFgFcCQFAqhKATEcCQBwKBwhqHkLYMgUgXorQAEopFUWEf0rsYX+kDL0+IAM6ZXxpGrUAJUEZvKNZYds1NObDByB+em197mWpUS6GCIJ6ygEAOREhxAAAREOd06qXSDkKOq/crtoqNluWAdV79HmmGeYce5aL36GDsJQcwW9VVKWbEpNF5xFmIBDSkzErq0WhqyVinJitbFjnKfISpnT5C9nOLirZ7F42WCQPcAA3N0wFJohXwsHE8kg9bQClpCIAFMIp2DJLBmpAWa1B5nzbmrGAVQCBoic6uJxRzjTtAHO6dS4yYTmxUS80SqG2HAAO2gA7fi1VYU6pqWNuMyZpJqQr3kOEAAkvofQpBiVhQfW+qkn6C3KJIRSqYnKUhoutf1VFVqaY8nojdQFwLQWYDljM79nC1B0EgKKkIdjAAJhMWLOTj+3XkafUTlJDf3hGbEQTs3Y21QYhPdXMJD1aawyDMpFYVTFPFzJ9Tsnhrz6zA7kzsVJ5mTJE7SODA4c6ICQ+h5IbiCUcwwyy7DvhcP4a/SQnBJGyN8s5bRgdDTKBNKY7SAT5s2McZ7EJr9OxhMwYnA+tQUhxCfVqoM/cTp/0AAkhmRdfcS3s+hob6BpQlmZSWwosdAIB4DEG5MQanUpBLzGkR/qNL4EDCmSEPoy25rsHnzgpcmUl+4vHYAkMOGp6jiG3nnA9d0WCsVoaofdUBEESXDNAuM2CgbqXmBtYxpZ+qfKqM2bswx6jc2XOWFzfmtFubCu0nA8Sh5qrF1JkwNEfAJAFAkApNFqL9XobRtSjSp7FwGsFeYJzKibHQzyEeEmDLu5ItEFMHNyAdbex7ehnQUVizAAX5Epd0SBWCAEvyDbZse2FUHCdn51IxMScoFJj4dbctHb27N2kGX4RlZywdm+JWHszea+5zAc2OsIc0913rQzRuDb0z1kbsUaVk1AEZkFU33tpaTMR0ji3HE0dWw5xjWd0eCe2wuaDIRyeVfk2pbHp32TndwVdhwt2gf3YS5ZJc9WXtPTew0GbX35g/aqn9ubgPgemEgGDiH+Wxsw7sKABHSPUeq/Nsj47i6l0rpzQWj6rMUjquQwjePOtkrXQvTkp9XbCm+GKTe5VUt9Z4UpC6jHrL+Gu+8EXpWcMpDdEi6s6k2fIGp4UOl4rOMXdhmayvMKm3MsRdjbFcwGQm3FmDc035vjtgVKUuqosMK4Xxqyuemtufr2lMJWP5ttTW30aV97GvIR/YDX6B36x4Rqc6Fp0cB9A/u/yFJwpyPuOaRU5p6Bun7POg+djDddXVMTXKdEsRXJpHHNnSldTLrFRXYRUWOK3VJOONNaFHRMMAdGXKzeXJxMA5Xd3TvCvAZR/MPG1X/ZTGDOnPLEsboJSMHegWXcjddWqIDBA6NK3JcQcNjVYG5JMAfCAvpEIYuG4Uuc/H9Ag6/crGAOTB/BcSvMMZ/NSQ8VVGoIrS/UrG/L/GkB9dnDTfnR+SEO4AEaSeuceG6euQtSUOAmEEEbeFlSAdA+bBg6zBXA/RzFXAHAgtjIg2Q37Eg/LHbN5ZQnXPLcIVVHJSncQz/CrJMbQqAzrTnFRSUYw3CB8UAJ8D5cw7rSwowseXCCww6WeOwhwzAuXFbVwvA9ONQaxNwLXP8AAvNDXXbGoDAygao/ALXU8eogIjoubdrOIp4GoGZJ4TXP8VlDCFIzMfufI8EHI7eFKFlYSHw13XvKiII9OAfAYoYkYp3KdcIrQ3XKkBCVVMkXo+nLvDXDdFguuFI3CUiPCEEJSCvJ4ZrL3U48HfWSHQ8APeHRHKdGoMkFHAdI3S7a7W7ZQhCI4k4yo33MI0Ab4oPX4sIgEoEi7E3G7DoiEqdKExmd42WP4hCeE4PfE3gZE0XVE0E2oskEki4O43eJE04vg/4kk6vGTJWc+GiPSJQvSZQpvI4XE+tVVPSQk345HNHakAfCPJQlQgQkvNSAYfvcvYgmUuGeUsQtQiQ2/e9YsRUpY+Q6kQ7F/KUkhFvF9VTOIjnPTZPOGe8VJa0i4LTWmSwceEXew+QFohbcjMo+zNw/jcvRY1MOQv7HYoImUiyF0VUo4UxAAIXCHRmgD0gAANVUEy4SQhYA/BrZI4YApgUA6AqQ7BpAqlsAL8SsNTQNRMwAEyLILVC1udzhkMQJjIDD9NDIxxpFcEEh7h4AEyKzQAnhpB2jQAEy0ULIdEOyEz3QCz4stl5ARhewJYhzH8EyiBpCdSAzfDeyEyd1OhJ9Q14l50/gGzgpmJmyjy2yG48Entuzeyng/AkRoAlY6AQgOskyF1OgJydhYyVp4yhzkzUzQB0zMz0BsyQhcz8ykBCziz9SDjX9VDSyoipCSFTEqyOyrdzU9CzzucvQARMLMxMpWxrzaQxMByQhhzut8KlwxzLz7S3lWwPypyR8m05zPzfy3zlydcdCYCLh6ztNLBGyQocLeKmyLzhRXsqLRK9M9yii3THCsCvS1snN2RqtZDvD1yq9eDy9ACAldso8iLKztydyDzMLhLqDih1UeLHThKcFqLBxo1GxCKaQxM7yzBHzny4jXyLKgpBkBLqCPyFy4zEy/ynyAKMzLBgLoAcy8zQACypAiz4BgijtTKcc38Ij1SEKwY5sQAEzrKJLbKhwlwSpC1cKRK0K7KuyeykxiKpBByyKVEKL2DUlKE0VWx4ZmrNx6KILpymKGAWLXy9yUzux2IPLjKfLhx2KYjkBzTdCiqhKBKcrSr8rGrUKko3kpKVqVERqTz8rpL3SnDsDcD1tKjWiFVByccWUtLyCtdQCMY2irrhxzqGigCdLhxTiOsI8eIZwKK8LlrJK7cRd/TbRAyVj5gID1jy9kdgzqCWS9KhzA0pBJ9PLbBZEzLBl5q2C7K8jyrMqwBbz7zXLJqphhreLZE/Kvy9IfykyUzgqXyKhCq3kpAUzAVeqmDN1Ga/AgNPB60UAqRMAkARh4rKqwAaQ+qSr0btriI0VkosbBa+ySKhzJaPltZvoHEpAXEPzgqJBwhoh7DzA8wilAhSlSkEyVaXEUgOoEyBb2QDS1IKhVVC9GYOsdtzr7akwTSMhLAdtTiMsAbJlLi9I0aHkMakpvqbLugg6aKQhkMpaLhH9gypaQdgLTiW8kUgSrE+VJ4eDGZ9aSkKg/hGUGoo6FF05kLS0A68rTKJa28tRWAUoHKZaYzFyLjmD9ABrHoRaSwqaDY1BRlrRKAVz04H1k6q7TiU0/SWarj6rw7QYvUYQlihQVI7IE76h+Di7KzS7J7xb7Sq77TOh4Fa6UyG6Ar5aq7W6hrx6W73QWQOb2jexubRc+a6BLaZbqQUzS6K7W8kZvp698FQ72C8jt76997TjozwgibLL+KtrfL3Qky49P75APzBqhzItO6hgQhuBe7+7GZ/MVQgtKAQtv6Ysu5vbz7RbA7N6QFAEkoAHGwNww6t64HIElwMofry77rK6GHAH5iXd56EoXjE6u4Otc0lbKlv6S0WzLAU8OGz0boFy+DYHWYR6BQYTTLhSQ8xTK5gS0TbsI9JGE9AH8thGC0UqcTfcI9VHkBQ8u4JTCoy66H37hHGGQRIsgA)
+
+With our main lemma out of the way, we immediately get `e ~ (nbeT α e)` and `completeness`:
+
+```lean
+-- e ~ nbeT α e
+theorem convrT_nbe {e : ExpT α} : e ~ (nbeT α e) :=
+  by
+  -- Hint: Use `all_R` and `R_convr_nbe`
+  sorry
+
+-- nbeT α e = nbeT α e' implies e ~ e'
+theorem completeness {e e' : ExpT α} : nbeT α e = nbeT α e' → e ~ e' :=
+  by
+  -- Hint: Use convrT_nbe
+  -- just like in Monoid-rewriting case.
+  sorry
+```
+[Try it!](https://live.lean-lang.org/#codez=LTAEDECcHsFsC5QAsAuKAOBneB6HBjTAOgEtp8iBTSnSgd00JwCYAGVgThwBMBPAIwBWlSDlgBDEgDsACuIA2sTJWCRKANxLLuRdNwBmAKBKx00SClABZcSiTyS/IgBVx+FCXyHjU7gFd3EnVKUGdeUEQw9EpDAB9QADlbCNDeONBxSBg6FLDQQCTCVILUw2hoqRLpfRIAD0gUgEZ2UAAiUEAlwgByVtAAXgA+DKzoOm9pf0Dg0ABRGvRc8MKomPiAaVAAb3FQfgWAX1BDw8QZudAACm2unY7u8QBKdIBlTe3d/H2jk9n588vbm7XfD3AH/a78EHXMHdYGPeIAQXQ8y2N0ivAOx0OPwuV26EOK2O2hWx/HSAC8RNAjtSaSlTvMkih0pgAh9abTvmdzoyAYy4aA1PgEq9Pl8sVzcRceddJQ9eckZY8ypQKj8fNUavJGs02oBcah6A1AiPQ3h8Ew8U3w0Ck6nqiEABcCbQCNwPsADQXbFOkGFc6e72gGQwE3xNT6LUbF1ovYbEKIT17QzslJWm31c6UEHp/mYXiwI4R/Yx0CUbpxs5OhNJxAp20XDN1zr+mtpkuZjPpFCQcRSTDOwshEvFzql+mgCuJ9nV621rMNpvTluNhtLwrNutt4f89bUguAJuBCzUUvHNuEy/Nd5XJ6A1+d1vrD/reJmavyXjuXfvAM3AUY2h7PF0/AF92uL0Dg2U9R3OQDrl3e4wLJI8zk/S8OWvBcLhee9QEfbDQDJZ9cIQ/VznCfV8P5cQkXzD9PhRXZ/3OYDulAzYPm4RDzxQmkp1THFM3xVd0POYELm4edeP+fURPOXZ9TE9JBQSAB9CkYD7KNNljUcK02fQOKlBVmIBUCJ1Qm9FNwkJ9T0sjKTbflFKUll8A+AsNI2Cp/0ZMCtOPDY9IY6UjJAuDTO4tCJIs/UrNAGyLmcj59Ske5MziipiKi4tcLSlL1VqbVWB6AA/A1BmbU1uEoPSwiU6QUBEBZimWdIwiIHlDUAVEJvHiTJsgyG5DWxaEdhBAB1i4arqhqiVSWqpHq+oIQqqqMiRZQ8zoz5zksNE5oWnEAQhDcFj26aQV2qbFoiXoLhQIhMF8IdHkMSq9KkPxYBEBQUh5Ykzlaxl0kKw1VOgdIpAAagaPpBgS3Dznez6uy1ZLvFegVKBIfRwn+NE2xOy6MnO0dtngXpDBwYAWt4NrbHdEIkyOQ1Ea+rUVlSIhepGfr+HdYT3X0EFDS8YAcEMfg0kOfBxGUXtxAnaXlESZJ2UNSgajcSwWeR4sFZlkIuZyN5DjVjX3GLIh9EwJk0ZWn5TrTUnUmJ9N9LlJZeAdjJ0gAAXWY3DVvV0wqTc5AG7gUB5kAMsILjvC41Cx8JtnQe5g8Zo5w9AABHUAY5TlL+R9l5jY+QOnjT9OM4jw8Y/OTD48x7GcS6fguhEl8K8ri4I/CWv6/OBOm8uFu25BF94cHnHxBbkEn07yvM4QmPKKwSg80uNa19AQ98JxTe83CciC9y+IfeNHnYqymHVtX9f7cJ4b8UFj05i97Z23iUH08DwrEA67NWTf0GOcBK88u5V1AJ5UAHVc6QKhiCQuFlti0kDopMB4Du6R1gQPSgQoJ6NyTpHVOIcMGZxzrXTKODE79RTvg6h3JbBdGnp0OUWdiEYJpJnKQhUY6MiIIKLBXCBSwJXutPet9s6QJBJAEE3Dj65Vtm9fgIRcbOzrG7F2hJzo3Unv1X0r9Cbv2eoYEAWUSqDlACYdADhKC9gANp2MoAAXScdsG6DiSwuPlvINeEgIq2iUhoBQgSc4oncgOEchIDiIBCOY7oPp9HoDfsWIWL8kmGKeto8WktLHzTUkgCc4wAgeGtMgCcCh5BKQAObQAUL2fAPjMj9QiaAcpUhPY1LqRkWxZQ9ZKxXmOUA+4S6gHYuIJSkAlLvAmUpMZ/BapIGvNwBZMMwp+CkPoaA8h2L33miIMKkAch2PEPMkgSB3T4GWWcpx3hTGxKHIcKxNjexSGUc0vokC3nv06IYHxsA/GYGgOs7gUhbG9jCakHyDz/ziGiWYh5hRXkGyyjdJFzTSzk0OBLCc6zNnbM+TER5eSqRIAaBOJA4gphIGYBxZJIQbq7P2t866/jJlBMqZQHOpKJyHNAHY6lNyTFgFcCQFAqhKATEcCQBwKBwhqHkLYMgUgXorQAEopFUWEf0rsYX+kDL0+IAM6ZXxpGrUAJUEZvKNZYds1NObDByB+em197mWpUS6GCIJ6ygEAOREhxAAAREOd06qXSDkKOq/crtoqNluWAdV79HmmGeYce5aL36GDsJQcwW9VVKWbEpNF5xFmIBDSkzErq0WhqyVinJitbFjnKfISpnT5C9nOLirZ7F42WCQPcAA3N0wFJohXwsHE8kg9bQClpCIAFMIp2DJLBmpAWa1B5nzbmrGAVQCBoic6uJxRzjTtAHO6dS4yYTmxUS80SqG2HAAO2gA7fi1VYU6pqWNuMyZpJqQr3kOEAAkvofQpBiVhQfW+qkn6C3KJIRSqYnKUhoutf1VFVqaY8nojdQFwLQWYDljM79nC1B0EgKKkIdjAAJhMWLOTj+3XkafUTlJDf3hGbEQTs3Y21QYhPdXMJD1aawyDMpFYVTFPFzJ9Tsnhrz6zA7kzsVJ5mTJE7SODA4c6ICQ+h5IbiCUcwwyy7DvhcP4a/SQnBJGyN8s5bRgdDTKBNKY7SAT5s2McZ7EJr9OxhMwYnA+tQUhxCfVqoM/cTp/0AAkhmRdfcS3s+hob6BpQlmZSWwosdAIB4DEG5MQanUpBLzGkR/qNL4EDCmSEPoy25rsHnzgpcmUl+4vHYAkMOGp6jiG3nnA9d0WCsVoaofdUBEESXDNAuM2CgbqXmBtYxpZ+qfKqM2bswx6jc2XOWFzfmtFubCu0nA8Sh5qrF1JkwNEfAJAFAkApNFqL9XobRtSjSp7FwGsFeYJzKibHQzyEeEmDLu5ItEFMHNyAdbex7ehnQUVizAAX5Epd0SBWCAEvyDbZse2FUHCdn51IxMScoFJj4dbctHb27N2kGX4RlZywdm+JWHszea+5zAc2OsIc0913rQzRuDb0z1kbsUaVk1AEZkFU33tpaTMR0ji3HE0dWw5xjWd0eCe2wuaDIRyeVfk2pbHp32TndwVdhwt2gf3YS5ZJc9WXtPTew0GbX35g/aqn9ubgPgemEgGDiH+Wxsw7sKABHSPUeq/Nsj47i6l0rpzQWj6rMUjquQwjePOtkrXQvTkp9XbCm+GKTe5VUt9Z4UpC6jHrL+Gu+8EXpWcMpDdEi6s6k2fIGp4UOl4rOMXdhmayvMKm3MsRdjbFcwGQm3FmDc035vjtgVKUuqosMK4Xxqyuemtufr2lMJWP5ttTW30aV97GvIR/YDX6B36x4Rqc6Fp0cB9A/u/yFJwpyPuOaRU5p6Bun7POg+djDddXVMTXKdEsRXJpHHNnSldTLrFRXYRUWOK3VJOONNaFHRMMAdGXKzeXJxMA5Xd3TvCvAZR/MPG1X/ZTGDOnPLEsboJSMHegWXcjddWqIDBA6NK3JcQcNjVYG5JMAfCAvpEIYuG4Uuc/H9Ag6/crGAOTB/BcSvMMZ/NSQ8VVGoIrS/UrG/L/GkB9dnDTfnR+SEO4AEaSeuceG6euQtSUOAmEEEbeFlSAdA+bBg6zBXA/RzFXAHAgtjIg2Q37Eg/LHbN5ZQnXPLcIVVHJSncQz/CrJMbQqAzrTnFRSUYw3CB8UAJ8D5cw7rSwowseXCCww6WeOwhwzAuXFbVwvA9ONQaxNwLXP8AAvNDXXbGoDAygao/ALXU8eogIjoubdrOIp4GoGZJ4TXP8VlDCFIzMfufI8EHI7eFKFlYSHw13XvKiII9OAfAYoYkYp3KdcIrQ3XKkBCVVMkXo+nLvDXDdFguuFI3CUiPCEEJSCvJ4ZrL3U48HfWSHQ8APeHRHKdGoMkFHAdI3S7a7W7ZQhCI4k4yo33MI0Ab4oPX4sIgEoEi7E3G7DoiEqdKExmd42WP4hCeE4PfE3gZE0XVE0E2oskEki4O43eJE04vg/4kk6vGTJWc+GiPSJQvSZQpvI4XE+tVVPSQk345HNHakAfCPJQlQgQkvNSAYfvcvYgmUuGeUsQtQiQ2/e9YsRUpY+Q6kQ7F/KUkhFvF9VTOIjnPTZPOGe8VJa0i4LTWmSwceEXew+QFohbcjMo+zNw/jcvRY1MOQv7HYoImUiyF0VUo4UxAAIXCHRmgD0gAANVUEy4SQhYA/BrZI4YApgUA6AqQ7BpAqlsAL8SsNTQNRMwAEyLILVC1udzhkMQJjIDD9NDIxxpFcEEh7h4AEyKzQAnhpB2jQAEy0ULIdEOyEz3QCz4stl5ARhewJYhzH8EyiBpCdSAzfDeyEyd1OhJ9Q14l50/gGzgpmJmyjy2yG48Entuzeyng/AkRoAlY6AQgOskyF1OgJydhYyVp4yhzkzUzQB0zMz0BsyQhcz8ykBCziz9SDjX9VDSyoipCSFTEqyOyrdzU9CzzucvQARMLMxMpWxrzaQxMByQhhzut8KlwxzLz7S3lWwPypyR8m05zPzfy3zlydcdCYCLh6ztNLBGyQocLeKmyLzhRXsqLRK9M9yii3THCsCvS1snN2RqtZDvD1yq9eDy9ACAldso8iLKztydyDzMLhLqDih1UeLHThKcFqLBxo1GxCKaQxM7yzBHzny4jXyLKgpBkBLqCPyFy4zEy/ynyAKMzLBgLoAcy8zQACypAiz4BgijtTKcc38Ij1SEKwY5sQAEzrKJLbKhwlwSpC1cKRK0K7KuyeykxiKpBByyKVEKL2DUlKE0VWx4ZmrNx6KILpymKGAWLXy9yUzux2IPLjKfLhx2KYjkBzTdCiqhKBKcrSr8rGrUKko3kpKVqVERqTz8rpL3SnDsDcD1tKjWiFVByccWUtLyCtdQCMY2irrhxzqGigCdLhxTiOsI8eIZwKK8LlrJK7cRd/TbRAyVj5gID1jy9kdgzqCWS9KhzA0pBJ9PLbBZEzLBl5q2C7K8jyrMqwBbz7zXLJqphhreLZE/Kvy9IfykyUzgqXyKhCq3kpAUzAVeqmDN1Ga/AgNPB60UAqRMAkARh4rKqwAaQ+qSr0btriI0VkosbBa+ySKhzJaPltZvoHEpAXEPzgqJBwhoh7DzA8wilAhSlSkEyVaXEUgOoEyBb2QDS1IKhVVC9GYOsdtzr7akwTSMhLAdtTiMsAbJlLi9I0aHkMakpvqbLugg6aKQhkMpaLhH9gypaQdgLTiW8kUgSrE+VJ4eDGZ9aSkKg/hGUGoo6FF05kLS0A68rTKJa28tRWAUoHKZaYzFyLjmD9ABrHoRaSwqaDY1BRlrRKAVz04H1k6q7TiU0/SWarj6rw7QYvUYQlihQVI7IE76h+Di7KzS7J7xb7Sq77TOh4Fa6UyG6Ar5aq7W6hrx6W73QWQOb2jexubRc+a6BLaZbqQUzS6K7W8kZvp698FQ72C8jt76997TjozwgibLL+KtrfL3Qky49P75APzBqhzItO6hgQhuBe7+7GZ/MVQgtKAQtv6Ysu5vbz7RbA7N6QFAEkoAHGwNww6t64HIElwMofry77rK6GHAH5iXd56EoXjE6u4Otc0lbKlv6S0WzLAU8OGz0boFy+DYHWYR6BQYTTLhSQ8xTK5gS0TbsI9JGE9AH8thGC0UqcTfcI9VHkBQ8u4JTCoy66H37hHGGQQYsR1U1VrdZM1s010FxnBgDF9tI4UK03H6w19PyJxTEIs6pEAABVJWBMufP8xBmB7oiq0XcwSANIEdJFZwBdRW5RbJqS8dete5RdDx1dNCJNQnFUKbBInJobN84oYpjFTPMJsACJ+aaJpWZsHxlTUAUxQQUK0ABwAAaxCGkGsGtGgBIG4HFQW0LNZL7onEBSyF4CAA)
+[Solution](https://live.lean-lang.org/#codez=LTAEDECcHsFsC5QAsAuKAOBneB6HBjTAOgEtp8iBTSnSgd00JwCYAGVgThwBMBPAIwBWlSDlgBDEgDsACuIA2sTJWCRKANxLLuRdNwBmAKBKx00SClABZcSiTyS/IgBVx+FCXyHjU7gFd3EnVKUGdeUEQw9EpDAB9QADlbCNDeONBxSBg6FLDQQCTCVILUw2hoqRLpfRIAD0gUgEZ2UAAiUEAlwgByVtAAXgA+DKzoOm9pf0Dg0ABRGvRc8MKomPiAaVAAb3FQfgWAX1BDw8QZudAACm2unY7u8QBKdIBlTe3d/H2jk9n588vbm7XfD3AH/a78EHXMHdYGPeIAQXQ8y2N0ivAOx0OPwuV26EOK2O2hWx/HSAC8RNAjtSaSlTvMkih0pgAh9abTvmdzoyAYy4aA1PgEq9Pl8sVzcRceddJQ9eckZY8ypQKj8fNUavJGs02oBcah6A1AiPQ3h8Ew8U3w0Ck6nqiEABcCbQCNwPsADQXbFOkGFc6e72gGQwE3xNT6LUbF1ovYbEKIT17QzslJWm31c6UEHp/mYXiwI4R/Yx0CUbpxs5OhNJxAp20XDN1zr+mtpkuZjPpFCQcRSTDOwshEvFzql+mgCuJ9nV621rMNpvTluNhtLwrNutt4f89bUguAJuBCzUUvHNuEy/Nd5XJ6A1+d1vrD/reJmavyXjuXfvAM3AUY2h7PF0/AF92uL0Dg2U9R3OQDrl3e4wLJI8zk/S8OWvBcLhee9QEfbDQDJZ9cIQ/VznCfV8P5cQkXzD9PhRXZ/3OYDulAzYPm4RDzxQmkp1THFM3xVd0POYELm4edeP+fURPOXZ9TE9JBQSAB9CkYD7KNNljUcK02fQOKlBVmIBUCJ1Qm9FNwkJ9T0sjKTbflFKUll8A+AsNI2Cp/0ZMCtOPDY9IY6UjJAuDTO4tCJIs/UrNAGyLmcj59Ske5MziipiKi4tcLSlL1VqbVWB6AA/A1BmbU1uEoPSwiU6QUBEBZimWdIwiIHlDUAVEJvHiTJsgyG5DWxaEdhBAB1i4arqhqiVSWqpHq+oIQqqqMiRZQ8zoz5zksNE5oWnEAQhDcFj26aQV2qbFoiXoLhQIhMF8IdHkMSq9KkPxYBEBQUh5Ykzlaxl0kKw1VOgdIpAAagaPpBgS3Dznez6uy1ZLvFegVKBIfRwn+NE2xOy6MnO0dtngXpDBwYAWt4NrbHdEIkyOQ1Ea+rUVlSIhepGfr+HdYT3X0EFDS8YAcEMfg0kOfBxGUXtxAnaXlESZJ2UNSgajcSwWeR4sFZlkIuZyN5DjVjX3GLIh9EwJk0ZWn5TrTUnUmJ9N9LlJZeAdjJ0gAAXWY3DVvV0wqTc5AG7gUB5kAMsILjvC41Cx8JtnQe5g8Zo5w9AABHUAY5TlL+R9l5jY+QOnjT9OM4jw8Y/OTD48x7GcS6fguhEl8K8ri4I/CWv6/OBOm8uFu25BF94cHnHxBbkEn07yvM4QmPKKwSg80uNa19AQ98JxTe83CciC9y+IfeNHnYqymHVtX9f7cJ4b8UFj05i97Z23iUH08DwrEA67NWTf0GOcBK88u5V1AJ5UAHVc6QKhiCQuFlti0kDopMB4Du6R1gQPSgQoJ6NyTpHVOIcMGZxzrXTKODE79RTvg6h3JbBdGnp0OUWdiEYJpJnKQhUY6MiIIKLBXCBSwJXutPet9s6QJBJAEE3Dj65Vtm9fgIRcbOzrG7F2hJzo3Unv1X0r9Cbv2eoYEAWUSqDlACYdADhKC9gANp2MoAAXScdsG6DiSwuPlvINeEgIq2iUhoBQgSc4oncgOEchIDiIBCOY7oPp9HoDfsWIWL8kmGKeto8WktLHzTUkgCc4wAgeGtMgCcCh5BKQAObQAUL2fAPjMj9QiaAcpUhPY1LqRkWxZQ9ZKxXmOUA+4S6gHYuIJSkAlLvAmUpMZ/BapIGvNwBZMMwp+CkPoaA8h2L33miIMKkAch2PEPMkgSB3T4GWWcpx3hTGxKHIcKxNjexSGUc0vokC3nv06IYHxsA/GYGgOs7gUhbG9jCakHyDz/ziGiWYh5hRXkGyyjdJFzTSzk0OBLCc6zNnbM+TER5eSqRIAaBOJA4gphIGYBxZJIQbq7P2t866/jJlBMqZQHOpKJyHNAHY6lNyTFgFcCQFAqhKATEcCQBwKBwhqHkLYMgUgXorQAEopFUWEf0rsYX+kDL0+IAM6ZXxpGrUAJUEZvKNZYds1NObDByB+em197mWpUS6GCIJ6ygEAOREhxAAAREOd06qXSDkKOq/crtoqNluWAdV79HmmGeYce5aL36GDsJQcwW9VVKWbEpNF5xFmIBDSkzErq0WhqyVinJitbFjnKfISpnT5C9nOLirZ7F42WCQPcAA3N0wFJohXwsHE8kg9bQClpCIAFMIp2DJLBmpAWa1B5nzbmrGAVQCBoic6uJxRzjTtAHO6dS4yYTmxUS80SqG2HAAO2gA7fi1VYU6pqWNuMyZpJqQr3kOEAAkvofQpBiVhQfW+qkn6C3KJIRSqYnKUhoutf1VFVqaY8nojdQFwLQWYDljM79nC1B0EgKKkIdjAAJhMWLOTj+3XkafUTlJDf3hGbEQTs3Y21QYhPdXMJD1aawyDMpFYVTFPFzJ9Tsnhrz6zA7kzsVJ5mTJE7SODA4c6ICQ+h5IbiCUcwwyy7DvhcP4a/SQnBJGyN8s5bRgdDTKBNKY7SAT5s2McZ7EJr9OxhMwYnA+tQUhxCfVqoM/cTp/0AAkhmRdfcS3s+hob6BpQlmZSWwosdAIB4DEG5MQanUpBLzGkR/qNL4EDCmSEPoy25rsHnzgpcmUl+4vHYAkMOGp6jiG3nnA9d0WCsVoaofdUBEESXDNAuM2CgbqXmBtYxpZ+qfKqM2bswx6jc2XOWFzfmtFubCu0nA8Sh5qrF1JkwNEfAJAFAkApNFqL9XobRtSjSp7FwGsFeYJzKibHQzyEeEmDLu5ItEFMHNyAdbex7ehnQUVizAAX5Epd0SBWCAEvyDbZse2FUHCdn51IxMScoFJj4dbctHb27N2kGX4RlZywdm+JWHszea+5zAc2OsIc0913rQzRuDb0z1kbsUaVk1AEZkFU33tpaTMR0ji3HE0dWw5xjWd0eCe2wuaDIRyeVfk2pbHp32TndwVdhwt2gf3YS5ZJc9WXtPTew0GbX35g/aqn9ubgPgemEgGDiH+Wxsw7sKABHSPUeq/Nsj47i6l0rpzQWj6rMUjquQwjePOtkrXQvTkp9XbCm+GKTe5VUt9Z4UpC6jHrL+Gu+8EXpWcMpDdEi6s6k2fIGp4UOl4rOMXdhmayvMKm3MsRdjbFcwGQm3FmDc035vjtgVKUuqosMK4Xxqyuemtufr2lMJWP5ttTW30aV97GvIR/YDX6B36x4Rqc6Fp0cB9A/u/yFJwpyPuOaRU5p6Bun7POg+djDddXVMTXKdEsRXJpHHNnSldTLrFRXYRUWOK3VJOONNaFHRMMAdGXKzeXJxMA5Xd3TvCvAZR/MPG1X/ZTGDOnPLEsboJSMHegWXcjddWqIDBA6NK3JcQcNjVYG5JMAfCAvpEIYuG4Uuc/H9Ag6/crGAOTB/BcSvMMZ/NSQ8VVGoIrS/UrG/L/GkB9dnDTfnR+SEO4AEaSeuceG6euQtSUOAmEEEbeFlSAdA+bBg6zBXA/RzFXAHAgtjIg2Q37Eg/LHbN5ZQnXPLcIVVHJSncQz/CrJMbQqAzrTnFRSUYw3CB8UAJ8D5cw7rSwowseXCCww6WeOwhwzAuXFbVwvA9ONQaxNwLXP8AAvNDXXbGoDAygao/ALXU8eogIjoubdrOIp4GoGZJ4TXP8VlDCFIzMfufI8EHI7eFKFlYSHw13XvKiII9OAfAYoYkYp3KdcIrQ3XKkBCVVMkXo+nLvDXDdFguuFI3CUiPCEEJSCvJ4ZrL3U48HfWSHQ8APeHRHKdGoMkFHAdI3S7a7W7ZQhCI4k4yo33MI0Ab4oPX4sIgEoEi7E3G7DoiEqdKExmd42WP4hCeE4PfE3gZE0XVE0E2oskEki4O43eJE04vg/4kk6vGTJWc+GiPSJQvSZQpvI4XE+tVVPSQk345HNHakAfCPJQlQgQkvNSAYfvcvYgmUuGeUsQtQiQ2/e9YsRUpY+Q6kQ7F/KUkhFvF9VTOIjnPTZPOGe8VJa0i4LTWmSwceEXew+QFohbcjMo+zNw/jcvRY1MOQv7HYoImUiyF0VUo4UxAAIXCHRmgD0gAANVUEy4SQhYA/BrZI4YApgUA6AqQ7BpAqlsAL8SsNTQNRMwAEyLILVC1udzhkMQJjIDD9NDIxxpFcEEh7h4AEyKzQAnhpB2jQAEy0ULIdEOyEz3QCz4stl5ARhewJYhzH8EyiBpCdSAzfDeyEyd1OhJ9Q14l50/gGzgpmJmyjy2yG48Entuzeyng/AkRoAlY6AQgOskyF1OgJydhYyVp4yhzkzUzQB0zMz0BsyQhcz8ykBCziz9SDjX9VDSyoipCSFTEqyOyrdzU9CzzucvQARMLMxMpWxrzaQxMByQhhzut8KlwxzLz7S3lWwPypyR8m05zPzfy3zlydcdCYCLh6ztNLBGyQocLeKmyLzhRXsqLRK9M9yii3THCsCvS1snN2RqtZDvD1yq9eDy9ACAldso8iLKztydyDzMLhLqDih1UeLHThKcFqLBxo1GxCKaQxM7yzBHzny4jXyLKgpBkBLqCPyFy4zEy/ynyAKMzLBgLoAcy8zQACypAiz4BgijtTKcc38Ij1SEKwY5sQAEzrKJLbKhwlwSpC1cKRK0K7KuyeykxiKpBByyKVEKL2DUlKE0VWx4ZmrNx6KILpymKGAWLXy9yUzux2IPLjKfLhx2KYjkBzTdCiqhKBKcrSr8rGrUKko3kpKVqVERqTz8rpL3SnDsDcD1tKjWiFVByccWUtLyCtdQCMY2irrhxzqGigCdLhxTiOsI8eIZwKK8LlrJK7cRd/TbRAyVj5gID1jy9kdgzqCWS9KhzA0pBJ9PLbBZEzLBl5q2C7K8jyrMqwBbz7zXLJqphhreLZE/Kvy9IfykyUzgqXyKhCq3kpAUzAVeqmDN1Ga/AgNPB60UAqRMAkARh4rKqwAaQ+qSr0btriI0VkosbBa+ySKhzJaPltZvoHEpAXEPzgqJBwhoh7DzA8wilAhSlSkEyVaXEUgOoEyBb2QDS1IKhVVC9GYOsdtzr7akwTSMhLAdtTiMsAbJlLi9I0aHkMakpvqbLugg6aKQhkMpaLhH9gypaQdgLTiW8kUgSrE+VJ4eDGZ9aSkKg/hGUGoo6FF05kLS0A68rTKJa28tRWAUoHKZaYzFyLjmD9ABrHoRaSwqaDY1BRlrRKAVz04H1k6q7TiU0/SWarj6rw7QYvUYQlihQVI7IE76h+Di7KzS7J7xb7Sq77TOh4Fa6UyG6Ar5aq7W6hrx6W73QWQOb2jexubRc+a6BLaZbqQUzS6K7W8kZvp698FQ72C8jt76997TjozwgibLL+KtrfL3Qky49P75APzBqhzItO6hgQhuBe7+7GZ/MVQgtKAQtv6Ysu5vbz7RbA7N6QFAEkoAHGwNww6t64HIElwMofry77rK6GHAH5iXd56EoXjE6u4Otc0lbKlv6S0WzLAU8OGz0boFy+DYHWYR6BQYTTLhSQ8xTK5gS0TbsI9JGE9AH8thGC0UqcTfcI9VHkBQ8u4JTCoy66H37hHGGQQYsR1U0vldY/k/FujNI3Y4UK03H6wRcLrgC58X0R0UD6U9NmVx1617lF0PHtgrQk1CcVQpsEj3kht0VihYmMVM9c8X9FLiHGjlFmdatWdDgSjPSXDvSKjtTBNuiWsgA)
+
+
+Finally, we have our main correctness theorem:
+```lean
+-- e ~ e' ↔ nbeT a e = nbeT a e'
+theorem correctnessT {e e' : ExpT a} : e ~ e' ↔ nbeT a e = nbeT a e' := ⟨soundness, completeness⟩
+```
+Like last time, Lean can now instantly decide any `a ~ b` problem through reflexivity:
+```lean
+-- I ⬝ x ~ x
+example {x : ExpT α}
+        : ((@I α β) ⬝ x)  ~  x := correctnessT.mpr rfl
+
+-- (B ⬝ x ⬝ y ⬝ z)  ~  (x ⬝ (y ⬝ z))
+example {x : ExpT (b ⇒' c)}
+        {y : ExpT (a ⇒' b)}
+        {z : ExpT a}
+        : (B ⬝ x ⬝ y ⬝ z)  ~  (x ⬝ (y ⬝ z)) := correctnessT.mpr rfl
+
+-- m + 0 ~ m
+example : (add m ⬝ .zero)  ~  m := correctnessT.mpr rfl
+
+-- m + (succ n) ~ succ (m + n)
+example : (add m ⬝ (.succ ⬝ n))  ~  (.succ ⬝ (add m ⬝ n)) := correctnessT.mpr rfl
+
+-- m * 0 ~ 0
+example : (mult m ⬝ .zero) ~ .zero := correctnessT.mpr rfl
+
+-- m * (succ n) ~ m + (m * n)
+example : (mult m ⬝ (.succ ⬝ n)) ~ ((add m) ⬝ (mult m ⬝ n)) := correctnessT.mpr rfl
+
+-- m ^ 0 ~ 1
+example : (power m ⬝ .zero) ~ (.succ ⬝ .zero) := correctnessT.mpr rfl
+
+-- m ^ (succ n) ~ m * (m ^ n)
+example : (power m ⬝ (.succ ⬝ n)) ~ ((mult m) ⬝ (power m ⬝ n)) := correctnessT.mpr rfl
+
+-- m ^ 3 ~ m * (m * m)
+example : (power m ⬝ (.succ ⬝ (.succ ⬝  (.succ ⬝ .zero))))  ~  (mult m ⬝ (mult m ⬝ m)) := correctnessT.mpr rfl
 ```
 
 
